<?xml version="1.0"?>
<rdf:RDF xmlns="http://purl.org/saws/ontology"
     xml:base="http://purl.org/saws/ontology"
     xmlns:dct="http://purl.org/dc/terms/"
     xmlns:owl="http://www.w3.org/2002/07/owl#"
     xmlns:rdf="http://www.w3.org/1999/02/22-rdf-syntax-ns#"
     xmlns:xml="http://www.w3.org/XML/1998/namespace"
     xmlns:xsd="http://www.w3.org/2001/XMLSchema#"
     xmlns:ecrm="http://erlangen-crm.org/current/"
     xmlns:rdfs="http://www.w3.org/2000/01/rdf-schema#"
     xmlns:efrbroo="http://erlangen-crm.org/efrbroo/">
    <owl:Ontology rdf:about="http://purl.org/saws/ontology">
        <rdfs:comment xml:lang="en">Ontology for the Sharing Ancient Wisdoms (SAWS) project, to represent the information and knowledge available in medieval gnomologia (collections of wise sayings). SAWS concentrates mainly on Ancient Greek and Arabic manuscripts containing wisdom literature. All class descriptions are provided by domain experts and the ontology has been developed through collaboration between these experts and ontology developers.</rdfs:comment>
        <rdfs:seeAlso rdf:datatype="http://www.w3.org/2001/XMLSchema#anyURI">http://www.ancientwisdoms.ac.uk</rdfs:seeAlso>
        <owl:priorVersion rdf:datatype="http://www.w3.org/2001/XMLSchema#double">1.4</owl:priorVersion>
        <owl:versionInfo xml:lang="en">Version 2.0. Produced after intensive discussions in Goettingen (September 2012) with SAWS project partners and various collaborators.</owl:versionInfo>
    </owl:Ontology>
    


    <!-- 
    ///////////////////////////////////////////////////////////////////////////////////////
    //
    // Object Properties
    //
    ///////////////////////////////////////////////////////////////////////////////////////
     -->

    


    <!-- http://erlangen-crm.org/current/P108_has_produced -->

    <owl:ObjectProperty rdf:about="http://erlangen-crm.org/current/P108_has_produced"/>
    


    <!-- http://erlangen-crm.org/current/P108i_was_produced_by -->

    <owl:ObjectProperty rdf:about="http://erlangen-crm.org/current/P108i_was_produced_by"/>
    


    <!-- http://erlangen-crm.org/current/P120_occurs_before -->

    <owl:ObjectProperty rdf:about="http://erlangen-crm.org/current/P120_occurs_before"/>
    


    <!-- http://erlangen-crm.org/current/P120i_occurs_after -->

    <owl:ObjectProperty rdf:about="http://erlangen-crm.org/current/P120i_occurs_after"/>
    


    <!-- http://erlangen-crm.org/current/P128_carries -->

    <owl:ObjectProperty rdf:about="http://erlangen-crm.org/current/P128_carries"/>
    


    <!-- http://erlangen-crm.org/current/P128i_is_carried_by -->

    <owl:ObjectProperty rdf:about="http://erlangen-crm.org/current/P128i_is_carried_by"/>
    


    <!-- http://erlangen-crm.org/current/P130_shows_features_of -->

    <owl:ObjectProperty rdf:about="http://erlangen-crm.org/current/P130_shows_features_of">
        <rdfs:subPropertyOf rdf:resource="http://purl.org/saws/ontology#isRelatedTo"/>
    </owl:ObjectProperty>
    


    <!-- http://erlangen-crm.org/current/P148_has_component -->

    <owl:ObjectProperty rdf:about="http://erlangen-crm.org/current/P148_has_component">
        <rdfs:subPropertyOf rdf:resource="http://purl.org/saws/ontology#hasMember"/>
    </owl:ObjectProperty>
    


    <!-- http://erlangen-crm.org/current/P14_carried_out_by -->

    <owl:ObjectProperty rdf:about="http://erlangen-crm.org/current/P14_carried_out_by"/>
    


    <!-- http://erlangen-crm.org/current/P14i_performed -->

    <owl:ObjectProperty rdf:about="http://erlangen-crm.org/current/P14i_performed"/>
    


    <!-- http://erlangen-crm.org/current/P16_used_specific_object -->

    <owl:ObjectProperty rdf:about="http://erlangen-crm.org/current/P16_used_specific_object"/>
    


    <!-- http://erlangen-crm.org/current/P16i_was_used_for -->

    <owl:ObjectProperty rdf:about="http://erlangen-crm.org/current/P16i_was_used_for"/>
    


    <!-- http://erlangen-crm.org/current/P46_is_composed_of -->

    <owl:ObjectProperty rdf:about="http://erlangen-crm.org/current/P46_is_composed_of"/>
    


    <!-- http://erlangen-crm.org/current/P46i_forms_part_of -->

    <owl:ObjectProperty rdf:about="http://erlangen-crm.org/current/P46i_forms_part_of"/>
    


    <!-- http://erlangen-crm.org/current/P51_has_former_or_current_owner -->

    <owl:ObjectProperty rdf:about="http://erlangen-crm.org/current/P51_has_former_or_current_owner"/>
    


    <!-- http://erlangen-crm.org/current/P51i_is_former_or_current_owner_of -->

    <owl:ObjectProperty rdf:about="http://erlangen-crm.org/current/P51i_is_former_or_current_owner_of"/>
    


    <!-- http://erlangen-crm.org/current/P53_has_former_or_current_location -->

    <owl:ObjectProperty rdf:about="http://erlangen-crm.org/current/P53_has_former_or_current_location"/>
    


    <!-- http://erlangen-crm.org/current/P53i_is_former_or_current_location_of -->

    <owl:ObjectProperty rdf:about="http://erlangen-crm.org/current/P53i_is_former_or_current_location_of"/>
    


    <!-- http://erlangen-crm.org/current/P67_refers_to -->

    <owl:ObjectProperty rdf:about="http://erlangen-crm.org/current/P67_refers_to"/>
    


    <!-- http://erlangen-crm.org/current/P67i_is_referred_to_by -->

    <owl:ObjectProperty rdf:about="http://erlangen-crm.org/current/P67i_is_referred_to_by"/>
    


    <!-- http://erlangen-crm.org/current/P72_has_language -->

    <owl:ObjectProperty rdf:about="http://erlangen-crm.org/current/P72_has_language"/>
    


    <!-- http://erlangen-crm.org/current/P72i_is_language_of -->

    <owl:ObjectProperty rdf:about="http://erlangen-crm.org/current/P72i_is_language_of">
        <owl:inverseOf rdf:resource="http://purl.org/saws/ontology#isInLanguage"/>
    </owl:ObjectProperty>
    


    <!-- http://erlangen-crm.org/current/P73_has_translation -->

    <owl:ObjectProperty rdf:about="http://erlangen-crm.org/current/P73_has_translation"/>
    


    <!-- http://erlangen-crm.org/current/P86i_contains -->

    <owl:ObjectProperty rdf:about="http://erlangen-crm.org/current/P86i_contains">
        <rdf:type rdf:resource="http://www.w3.org/2002/07/owl#TransitiveProperty"/>
        <rdfs:domain rdf:resource="http://erlangen-crm.org/current/E33_Linguistic_Object"/>
        <rdfs:range rdf:resource="http://erlangen-crm.org/current/E33_Linguistic_Object"/>
    </owl:ObjectProperty>
    


    <!-- http://erlangen-crm.org/current/P94_has_created -->

    <owl:ObjectProperty rdf:about="http://erlangen-crm.org/current/P94_has_created"/>
    


    <!-- http://erlangen-crm.org/current/P94i_was_created_by -->

    <owl:ObjectProperty rdf:about="http://erlangen-crm.org/current/P94i_was_created_by"/>
    


    <!-- http://erlangen-crm.org/efrbroo/R17_created -->

    <owl:ObjectProperty rdf:about="http://erlangen-crm.org/efrbroo/R17_created"/>
    


    <!-- http://erlangen-crm.org/efrbroo/R17i_was_created_by -->

    <owl:ObjectProperty rdf:about="http://erlangen-crm.org/efrbroo/R17i_was_created_by"/>
    


    <!-- http://erlangen-crm.org/efrbroo/R18_created -->

    <owl:ObjectProperty rdf:about="http://erlangen-crm.org/efrbroo/R18_created"/>
    


    <!-- http://erlangen-crm.org/efrbroo/R18i_was_created_by -->

    <owl:ObjectProperty rdf:about="http://erlangen-crm.org/efrbroo/R18i_was_created_by"/>
    


    <!-- http://erlangen-crm.org/efrbroo/R5_has_component -->

    <owl:ObjectProperty rdf:about="http://erlangen-crm.org/efrbroo/R5_has_component"/>
    


    <!-- http://erlangen-crm.org/efrbroo/R5i_is_component_of -->

    <owl:ObjectProperty rdf:about="http://erlangen-crm.org/efrbroo/R5i_is_component_of"/>
    


    <!-- http://purl.org/saws/ontology#areMarginaliaOn -->

    <owl:ObjectProperty rdf:about="http://purl.org/saws/ontology#areMarginaliaOn">
        <rdfs:subPropertyOf rdf:resource="http://purl.org/saws/ontology#refersTo"/>
        <owl:inverseOf rdf:resource="http://purl.org/saws/ontology#hasMarginalia"/>
        <rdfs:domain rdf:resource="http://purl.org/saws/ontology#Marginalia"/>
        <rdfs:range rdf:resource="http://purl.org/saws/ontology#OriginalMaterial"/>
        <rdfs:comment xml:lang="en">To indicate that Marginalia have been written on the manuscript,e .g. in the margins</rdfs:comment>
        <rdfs:label xml:lang="en">are marginalia on</rdfs:label>
    </owl:ObjectProperty>
    


    <!-- http://purl.org/saws/ontology#contains -->

    <owl:ObjectProperty rdf:about="http://purl.org/saws/ontology#contains">
        <rdfs:subPropertyOf rdf:resource="http://erlangen-crm.org/current/P86i_contains"/>
        <rdfs:subPropertyOf rdf:resource="http://purl.org/saws/ontology#isRelatedTo"/>
        <owl:inverseOf rdf:resource="http://purl.org/saws/ontology#fallsWithin"/>
    </owl:ObjectProperty>
    


    <!-- http://purl.org/saws/ontology#containsTextInLanguage -->

    <owl:ObjectProperty rdf:about="http://purl.org/saws/ontology#containsTextInLanguage">
        <rdfs:domain>
            <owl:Class>
                <owl:unionOf rdf:parseType="Collection">
                    <rdf:Description rdf:about="http://purl.org/saws/ontology#ManuscriptPart"/>
                    <rdf:Description rdf:about="http://purl.org/saws/ontology#PhysicalManuscript"/>
                    <rdf:Description rdf:about="http://purl.org/saws/ontology#ReconstructedManuscript"/>
                </owl:unionOf>
            </owl:Class>
        </rdfs:domain>
        <rdfs:range rdf:resource="http://erlangen-crm.org/current/E56_Language"/>
        <owl:propertyChainAxiom rdf:parseType="Collection">
            <rdf:Description rdf:about="http://erlangen-crm.org/current/P128_carries"/>
            <rdf:Description rdf:about="http://purl.org/saws/ontology#isInLanguage"/>
        </owl:propertyChainAxiom>
    </owl:ObjectProperty>
    


    <!-- http://purl.org/saws/ontology#decorationAddedBy -->

    <owl:ObjectProperty rdf:about="http://purl.org/saws/ontology#decorationAddedBy">
        <rdfs:subPropertyOf rdf:resource="http://purl.org/saws/ontology#isRelatedTo"/>
        <rdfs:domain rdf:resource="http://purl.org/saws/ontology#DecorativeItem"/>
        <rdfs:range rdf:resource="http://erlangen-crm.org/current/E21_Person"/>
        <owl:propertyChainAxiom rdf:parseType="Collection">
            <rdf:Description rdf:about="http://erlangen-crm.org/current/P94i_was_created_by"/>
            <rdf:Description rdf:about="http://erlangen-crm.org/current/P14_carried_out_by"/>
        </owl:propertyChainAxiom>
        <rdfs:comment xml:lang="en">A DecorativeItem has been physically added onto the manuscript by a Person

NB to represent marginalia notes (text) physically written in the margins of the manuscript, use: Marginalia marginaliaAddedBy Scribe @en</rdfs:comment>
        <rdfs:label xml:lang="en">decoration added by</rdfs:label>
        <rdfs:seeAlso xml:lang="en">Marginalia marginaliaAddedBy Scribe</rdfs:seeAlso>
    </owl:ObjectProperty>
    


    <!-- http://purl.org/saws/ontology#fallsWithin -->

    <owl:ObjectProperty rdf:about="http://purl.org/saws/ontology#fallsWithin">
        <rdfs:subPropertyOf rdf:resource="http://purl.org/saws/ontology#isRelatedTo"/>
    </owl:ObjectProperty>
    


    <!-- http://purl.org/saws/ontology#follows -->

    <owl:ObjectProperty rdf:about="http://purl.org/saws/ontology#follows">
        <rdfs:subPropertyOf rdf:resource="http://purl.org/saws/ontology#isRelatedTo"/>
        <owl:inverseOf rdf:resource="http://purl.org/saws/ontology#precedes"/>
        <rdf:type rdf:resource="http://www.w3.org/2002/07/owl#TransitiveProperty"/>
        <rdfs:domain rdf:resource="http://erlangen-crm.org/current/E33_Linguistic_Object"/>
        <rdfs:range rdf:resource="http://erlangen-crm.org/current/E33_Linguistic_Object"/>
        <rdfs:comment xml:lang="en">A Section/ContentItem/CollectionInstance comes after another Section/ContentItem/CollectionInstance in the document</rdfs:comment>
        <rdfs:label xml:lang="en">follows</rdfs:label>
    </owl:ObjectProperty>
    


    <!-- http://purl.org/saws/ontology#formsPartOf -->

    <owl:ObjectProperty rdf:about="http://purl.org/saws/ontology#formsPartOf">
        <rdfs:subPropertyOf rdf:resource="http://erlangen-crm.org/current/P46i_forms_part_of"/>
        <rdfs:subPropertyOf rdf:resource="http://purl.org/saws/ontology#isRelatedTo"/>
        <owl:inverseOf rdf:resource="http://purl.org/saws/ontology#hasPart"/>
        <rdfs:comment xml:lang="en">Physical Manuscripts can be composed of many Manuscript Parts – this relationship would be stated once for each part. This relationship can be used both for existing Manuscript Parts or for Manuscript Parts which used to be parts of a manuscript</rdfs:comment>
        <rdfs:label xml:lang="en">forms part of</rdfs:label>
    </owl:ObjectProperty>
    


    <!-- http://purl.org/saws/ontology#hasAddedMarginalia -->

    <owl:ObjectProperty rdf:about="http://purl.org/saws/ontology#hasAddedMarginalia">
        <rdfs:subPropertyOf rdf:resource="http://purl.org/saws/ontology#isRelatedTo"/>
        <owl:inverseOf rdf:resource="http://purl.org/saws/ontology#marginaliaAddedBy"/>
        <rdfs:domain rdf:resource="http://purl.org/saws/ontology#Scribe"/>
        <rdfs:range rdf:resource="http://purl.org/saws/ontology#Marginalia"/>
        <owl:propertyChainAxiom rdf:parseType="Collection">
            <rdf:Description rdf:about="http://erlangen-crm.org/current/P14i_performed"/>
            <rdf:Description rdf:about="http://erlangen-crm.org/current/P94_has_created"/>
        </owl:propertyChainAxiom>
        <rdfs:comment xml:lang="en">A Scribe has physically added Marginalia onto a manuscript.

NB to represent where a modern-day scholar/editor makes a comment, not written onto the manuscript, use: Editor hasMadeComment Comment </rdfs:comment>
        <rdfs:label xml:lang="en">has added marginalia</rdfs:label>
        <rdfs:seeAlso xml:lang="en">Person hasWritten LinguisticObject
Editor hasMadeComment Comment</rdfs:seeAlso>
    </owl:ObjectProperty>
    


    <!-- http://purl.org/saws/ontology#hasAncestor -->

    <owl:ObjectProperty rdf:about="http://purl.org/saws/ontology#hasAncestor">
        <rdfs:subPropertyOf rdf:resource="http://purl.org/saws/ontology#isInSameFamilyAs"/>
        <owl:inverseOf rdf:resource="http://purl.org/saws/ontology#isAncestorOf"/>
    </owl:ObjectProperty>
    


    <!-- http://purl.org/saws/ontology#hasChild -->

    <owl:ObjectProperty rdf:about="http://purl.org/saws/ontology#hasChild">
        <rdfs:subPropertyOf rdf:resource="http://purl.org/saws/ontology#hasDescendant"/>
        <owl:inverseOf rdf:resource="http://purl.org/saws/ontology#isChildOf"/>
        <rdfs:comment xml:lang="en">The parent OriginalMaterial is a direct source for the production of part or all of the child OriginalMaterial</rdfs:comment>
        <rdfs:label xml:lang="en">hasChild</rdfs:label>
    </owl:ObjectProperty>
    


    <!-- http://purl.org/saws/ontology#hasComment -->

    <owl:ObjectProperty rdf:about="http://purl.org/saws/ontology#hasComment">
        <rdfs:subPropertyOf rdf:resource="http://purl.org/saws/ontology#isReferencedBy"/>
        <owl:inverseOf rdf:resource="http://purl.org/saws/ontology#isCommentOn"/>
        <rdfs:domain rdf:resource="http://erlangen-crm.org/current/E1_CRM_Entity"/>
        <rdfs:range rdf:resource="http://purl.org/saws/ontology#Comment"/>
        <rdfs:comment xml:lang="en">To indicate that something has been commented about in an editorial Comment </rdfs:comment>
        <rdfs:label xml:lang="en">has comment</rdfs:label>
    </owl:ObjectProperty>
    


    <!-- http://purl.org/saws/ontology#hasComponent -->

    <owl:ObjectProperty rdf:about="http://purl.org/saws/ontology#hasComponent">
        <rdfs:subPropertyOf rdf:resource="http://erlangen-crm.org/efrbroo/R5_has_component"/>
        <owl:inverseOf rdf:resource="http://purl.org/saws/ontology#isComponentOf"/>
        <rdfs:domain rdf:resource="http://erlangen-crm.org/efrbroo/F2_Expression"/>
        <rdfs:range rdf:resource="http://erlangen-crm.org/efrbroo/F2_Expression"/>
    </owl:ObjectProperty>
    


    <!-- http://purl.org/saws/ontology#hasDescendant -->

    <owl:ObjectProperty rdf:about="http://purl.org/saws/ontology#hasDescendant">
        <rdfs:subPropertyOf rdf:resource="http://purl.org/saws/ontology#isInSameFamilyAs"/>
        <owl:inverseOf rdf:resource="http://purl.org/saws/ontology#isDescendantOf"/>
        <rdf:type rdf:resource="http://www.w3.org/2002/07/owl#TransitiveProperty"/>
        <owl:propertyChainAxiom rdf:parseType="Collection">
            <rdf:Description rdf:about="http://purl.org/saws/ontology#hasChild"/>
            <rdf:Description rdf:about="http://purl.org/saws/ontology#hasDescendant"/>
        </owl:propertyChainAxiom>
        <rdfs:comment xml:lang="en">An ancestor OriginalMaterial is a source material (direct or indirect) for the production of part or all of the descendant OriginalMaterial</rdfs:comment>
        <rdfs:label xml:lang="en">has descendant</rdfs:label>
    </owl:ObjectProperty>
    


    <!-- http://purl.org/saws/ontology#hasMadeComment -->

    <owl:ObjectProperty rdf:about="http://purl.org/saws/ontology#hasMadeComment">
        <rdfs:subPropertyOf rdf:resource="http://purl.org/saws/ontology#isRelatedTo"/>
        <rdfs:domain rdf:resource="http://purl.org/saws/ontology#Editor"/>
        <rdfs:range rdf:resource="http://purl.org/saws/ontology#Comment"/>
        <owl:propertyChainAxiom rdf:parseType="Collection">
            <rdf:Description rdf:about="http://erlangen-crm.org/current/P14i_performed"/>
            <rdf:Description rdf:about="http://erlangen-crm.org/current/P94_has_created"/>
        </owl:propertyChainAxiom>
        <rdfs:comment xml:lang="en">A modern-day scholar/editor has made a comment. 

NB to represent scribes physically writing marginalia on the manuscript, use: Scribe hasAddedMarginalia.&quot;@en</rdfs:comment>
        <rdfs:label xml:lang="en">has made comment</rdfs:label>
        <rdfs:seeAlso xml:lang="en">Person hasWritten LinguisticObject
Scribe hasAddedMarginalia Marginalia </rdfs:seeAlso>
    </owl:ObjectProperty>
    


    <!-- http://purl.org/saws/ontology#hasMarginalia -->

    <owl:ObjectProperty rdf:about="http://purl.org/saws/ontology#hasMarginalia">
        <rdfs:subPropertyOf rdf:resource="http://purl.org/saws/ontology#isReferencedBy"/>
        <rdfs:domain rdf:resource="http://purl.org/saws/ontology#OriginalMaterial"/>
        <rdfs:range rdf:resource="http://purl.org/saws/ontology#Marginalia"/>
        <rdfs:comment xml:lang="en">To indicate that a manuscript has had Marginalia written on it, e.g. in the margins</rdfs:comment>
        <rdfs:label xml:lang="en">has marginalia</rdfs:label>
    </owl:ObjectProperty>
    


    <!-- http://purl.org/saws/ontology#hasMember -->

    <owl:ObjectProperty rdf:about="http://purl.org/saws/ontology#hasMember">
        <rdfs:subPropertyOf rdf:resource="http://purl.org/saws/ontology#isRelatedTo"/>
        <owl:inverseOf rdf:resource="http://purl.org/saws/ontology#isMemberOf"/>
        <rdf:type rdf:resource="http://www.w3.org/2002/07/owl#TransitiveProperty"/>
        <rdf:type rdf:resource="http://www.w3.org/2002/07/owl#ReflexiveProperty"/>
        <rdfs:domain rdf:resource="http://erlangen-crm.org/current/E1_CRM_Entity"/>
        <rdfs:range rdf:resource="http://erlangen-crm.org/current/E1_CRM_Entity"/>
        <rdfs:comment xml:lang="en">We use hasMember to indicate:
- A Family contains the specified original material (i.e. one
produced by Scribe transcription rather than being edited in modern times)
- An Institution has as a member this Person</rdfs:comment>
        <rdfs:label xml:lang="en">has member</rdfs:label>
        <rdfs:seeAlso xml:lang="en">dct:hasPart
efrbroo:R10_has_member
ecrm:P107_has_current_or_former_member</rdfs:seeAlso>
    </owl:ObjectProperty>
    


    <!-- http://purl.org/saws/ontology#hasOwned -->

    <owl:ObjectProperty rdf:about="http://purl.org/saws/ontology#hasOwned">
        <rdfs:subPropertyOf rdf:resource="http://purl.org/saws/ontology#isRelatedTo"/>
        <owl:inverseOf rdf:resource="http://purl.org/saws/ontology#ownedBy"/>
        <rdfs:domain>
            <owl:Class>
                <owl:unionOf rdf:parseType="Collection">
                    <rdf:Description rdf:about="http://erlangen-crm.org/current/E21_Person"/>
                    <rdf:Description rdf:about="http://purl.org/saws/ontology#Institution"/>
                </owl:unionOf>
            </owl:Class>
        </rdfs:domain>
        <rdfs:range rdf:resource="http://purl.org/saws/ontology#Material"/>
        <owl:propertyChainAxiom rdf:parseType="Collection">
            <rdf:Description rdf:about="http://erlangen-crm.org/current/P51i_is_former_or_current_owner_of"/>
            <rdf:Description rdf:about="http://erlangen-crm.org/current/P128_carries"/>
        </owl:propertyChainAxiom>
        <rdfs:comment xml:lang="en">A Person has owned (either currently or in the past) the Material of Interest. This would normally be based on a specific statement/mark of ownership.

[nb this will always need a date?]</rdfs:comment>
        <rdfs:label xml:lang="en">has owned</rdfs:label>
    </owl:ObjectProperty>
    


    <!-- http://purl.org/saws/ontology#hasParent -->

    <owl:ObjectProperty rdf:about="http://purl.org/saws/ontology#hasParent">
        <rdfs:subPropertyOf rdf:resource="http://purl.org/saws/ontology#hasAncestor"/>
        <owl:inverseOf rdf:resource="http://purl.org/saws/ontology#isParentOf"/>
    </owl:ObjectProperty>
    


    <!-- http://purl.org/saws/ontology#hasPart -->

    <owl:ObjectProperty rdf:about="http://purl.org/saws/ontology#hasPart">
        <rdfs:subPropertyOf rdf:resource="http://erlangen-crm.org/current/P46_is_composed_of"/>
        <rdfs:subPropertyOf rdf:resource="http://purl.org/saws/ontology#isRelatedTo"/>
        <rdfs:comment xml:lang="en">Physical Manuscripts can be composed of many Manuscript Parts – this relationship would be stated once for each part. This relationship can be used both for existing Manuscript Parts or for Manuscript Parts which used to be parts of a manuscript</rdfs:comment>
        <rdfs:label xml:lang="en">has part</rdfs:label>
    </owl:ObjectProperty>
    


    <!-- http://purl.org/saws/ontology#hasUsed -->

    <owl:ObjectProperty rdf:about="http://purl.org/saws/ontology#hasUsed">
        <rdfs:subPropertyOf rdf:resource="http://purl.org/saws/ontology#isRelatedTo"/>
        <owl:inverseOf rdf:resource="http://purl.org/saws/ontology#usedBy"/>
        <rdfs:domain rdf:resource="http://erlangen-crm.org/efrbroo/F10_Person"/>
        <rdfs:range rdf:resource="http://purl.org/saws/ontology#OriginalMaterial"/>
        <owl:propertyChainAxiom rdf:parseType="Collection">
            <rdf:Description rdf:about="http://erlangen-crm.org/current/P14i_performed"/>
            <rdf:Description rdf:about="http://erlangen-crm.org/current/P16_used_specific_object"/>
        </owl:propertyChainAxiom>
        <rdfs:comment xml:lang="en">A Person has used (either currently or in the past) the OriginalMaterial in their work.

[nb this will always need a date?]</rdfs:comment>
        <rdfs:label xml:lang="en">has used</rdfs:label>
    </owl:ObjectProperty>
    


    <!-- http://purl.org/saws/ontology#hasWritten -->

    <owl:ObjectProperty rdf:about="http://purl.org/saws/ontology#hasWritten">
        <rdfs:subPropertyOf rdf:resource="http://purl.org/saws/ontology#isRelatedTo"/>
        <owl:inverseOf rdf:resource="http://purl.org/saws/ontology#isWrittenBy"/>
        <rdfs:domain rdf:resource="http://erlangen-crm.org/current/E21_Person"/>
        <rdfs:range rdf:resource="http://erlangen-crm.org/current/E33_Linguistic_Object"/>
        <owl:propertyChainAxiom rdf:parseType="Collection">
            <rdf:Description rdf:about="http://erlangen-crm.org/current/P14i_performed"/>
            <rdf:Description rdf:about="http://erlangen-crm.org/current/P94_has_created"/>
        </owl:propertyChainAxiom>
        <rdfs:comment xml:lang="en">A Person has written (or has transcribed) a LinguisticObject.
NB This also includes:
Editor hasWritten Comment
Scribe hasWritten Marginalia</rdfs:comment>
        <rdfs:label xml:lang="en">has written</rdfs:label>
        <rdfs:seeAlso xml:lang="en">Editor hasMadeComment Comment
Scribe hasAddedMarginalia Marginalia</rdfs:seeAlso>
    </owl:ObjectProperty>
    


    <!-- http://purl.org/saws/ontology#isAncestorOf -->

    <owl:ObjectProperty rdf:about="http://purl.org/saws/ontology#isAncestorOf">
        <rdfs:subPropertyOf rdf:resource="http://purl.org/saws/ontology#isInSameFamilyAs"/>
        <rdf:type rdf:resource="http://www.w3.org/2002/07/owl#TransitiveProperty"/>
        <owl:propertyChainAxiom rdf:parseType="Collection">
            <rdf:Description rdf:about="http://purl.org/saws/ontology#isParentOf"/>
            <rdf:Description rdf:about="http://purl.org/saws/ontology#isAncestorOf"/>
        </owl:propertyChainAxiom>
        <rdfs:comment xml:lang="en">An ancestor OriginalMaterial is a source material (direct or indirect) for the production of part or all of the descendant OriginalMaterial</rdfs:comment>
        <rdfs:label xml:lang="en">is ancestor of</rdfs:label>
    </owl:ObjectProperty>
    


    <!-- http://purl.org/saws/ontology#isAttributedAuthorOf -->

    <owl:ObjectProperty rdf:about="http://purl.org/saws/ontology#isAttributedAuthorOf">
        <rdfs:subPropertyOf rdf:resource="http://purl.org/saws/ontology#hasWritten"/>
        <owl:inverseOf rdf:resource="http://purl.org/saws/ontology#isAttributedToAuthor"/>
        <rdfs:domain rdf:resource="http://purl.org/saws/ontology#AttributedAuthor"/>
        <rdfs:range>
            <owl:Class>
                <owl:intersectionOf rdf:parseType="Collection">
                    <rdf:Description rdf:about="http://erlangen-crm.org/current/E33_Linguistic_Object"/>
                    <owl:Class>
                        <owl:complementOf rdf:resource="http://purl.org/saws/ontology#Edition"/>
                    </owl:Class>
                </owl:intersectionOf>
            </owl:Class>
        </rdfs:range>
        <rdfs:comment xml:lang="en">An author has been attributed as the author of this LinguisticObject (any Linguistic Object except Edition)</rdfs:comment>
        <rdfs:label xml:lang="en">is attributed author of</rdfs:label>
    </owl:ObjectProperty>
    


    <!-- http://purl.org/saws/ontology#isAttributedToAuthor -->

    <owl:ObjectProperty rdf:about="http://purl.org/saws/ontology#isAttributedToAuthor">
        <rdfs:subPropertyOf rdf:resource="http://purl.org/saws/ontology#isWrittenBy"/>
        <rdfs:domain>
            <owl:Class>
                <owl:intersectionOf rdf:parseType="Collection">
                    <rdf:Description rdf:about="http://erlangen-crm.org/current/E33_Linguistic_Object"/>
                    <owl:Class>
                        <owl:complementOf rdf:resource="http://purl.org/saws/ontology#Edition"/>
                    </owl:Class>
                </owl:intersectionOf>
            </owl:Class>
        </rdfs:domain>
        <rdfs:range rdf:resource="http://purl.org/saws/ontology#AttributedAuthor"/>
        <rdfs:comment xml:lang="en">A LinguisticObject (except Edition) is attributed to this AttributedAuthor</rdfs:comment>
        <rdfs:label xml:lang="en">is attributed to author</rdfs:label>
    </owl:ObjectProperty>
    


    <!-- http://purl.org/saws/ontology#isBasedOn -->

    <owl:ObjectProperty rdf:about="http://purl.org/saws/ontology#isBasedOn">
        <rdfs:subPropertyOf rdf:resource="http://purl.org/saws/ontology#isRelatedTo"/>
        <owl:inverseOf rdf:resource="http://purl.org/saws/ontology#isSourceFor"/>
        <rdfs:domain rdf:resource="http://purl.org/saws/ontology#Edition"/>
        <rdfs:range rdf:resource="http://erlangen-crm.org/current/E33_Linguistic_Object"/>
        <rdfs:comment xml:lang="en">An edition is based upon one or more textual materials (manuscripts, collections etc). One &lt;relation&gt; per each textual material)</rdfs:comment>
        <rdfs:label xml:lang="en">is based on</rdfs:label>
    </owl:ObjectProperty>
    


    <!-- http://purl.org/saws/ontology#isBySameScribeAs -->

    <owl:ObjectProperty rdf:about="http://purl.org/saws/ontology#isBySameScribeAs">
        <rdfs:subPropertyOf rdf:resource="http://purl.org/saws/ontology#isRelatedTo"/>
        <rdf:type rdf:resource="http://www.w3.org/2002/07/owl#SymmetricProperty"/>
        <rdf:type rdf:resource="http://www.w3.org/2002/07/owl#TransitiveProperty"/>
        <rdfs:domain>
            <owl:Class>
                <owl:unionOf rdf:parseType="Collection">
                    <rdf:Description rdf:about="http://purl.org/saws/ontology#ManuscriptPart"/>
                    <rdf:Description rdf:about="http://purl.org/saws/ontology#PhysicalManuscript"/>
                    <rdf:Description rdf:about="http://purl.org/saws/ontology#ReconstructedManuscript"/>
                </owl:unionOf>
            </owl:Class>
        </rdfs:domain>
        <rdfs:range>
            <owl:Class>
                <owl:unionOf rdf:parseType="Collection">
                    <rdf:Description rdf:about="http://purl.org/saws/ontology#ManuscriptPart"/>
                    <rdf:Description rdf:about="http://purl.org/saws/ontology#PhysicalManuscript"/>
                    <rdf:Description rdf:about="http://purl.org/saws/ontology#ReconstructedManuscript"/>
                </owl:unionOf>
            </owl:Class>
        </rdfs:range>
        <rdfs:comment xml:lang="en">The two manuscripts (or parts of the manuscripts) have been copied/produced by the same Person</rdfs:comment>
        <rdfs:label xml:lang="en">is by same scribe as</rdfs:label>
        <rdfs:seeAlso xml:lang="en">Person hasWritten LinguisticObject
LinguisticObject isWrittenBy Person

PhysicalManuscript/ReconstructedManuscript/ManuscriptPart isFromSamePlaceAs PhysicalManuscript/ReconstructedManuscript/ManuscriptPart</rdfs:seeAlso>
    </owl:ObjectProperty>
    


    <!-- http://purl.org/saws/ontology#isChildOf -->

    <owl:ObjectProperty rdf:about="http://purl.org/saws/ontology#isChildOf">
        <rdfs:subPropertyOf rdf:resource="http://purl.org/saws/ontology#isDescendantOf"/>
        <rdfs:comment xml:lang="en">The parent OriginalMaterial is a direct source for the production of part or all of the child OriginalMaterial</rdfs:comment>
        <rdfs:label xml:lang="en">is child of</rdfs:label>
    </owl:ObjectProperty>
    


    <!-- http://purl.org/saws/ontology#isCloseRenderingOf -->

    <owl:ObjectProperty rdf:about="http://purl.org/saws/ontology#isCloseRenderingOf">
        <rdfs:subPropertyOf rdf:resource="http://purl.org/saws/ontology#isVariantOf"/>
        <rdfs:domain rdf:resource="http://erlangen-crm.org/current/E33_Linguistic_Object"/>
        <rdfs:range rdf:resource="http://erlangen-crm.org/current/E33_Linguistic_Object"/>
        <rdfs:comment xml:lang="en">From one dialect or genre into another. This property specifies the source and target LinguisticObject involved (respectively) when rendering one LinguisticObject instance to express it in a related but different way (not necessarily in a different Language), resulting in a new LinguisticObject e.g. poetry into prose, or from one dialect to another, or a paraphrase being made.  This property indicates that the new LinguisticObject is a close rendering of the original LinguisticObject.

For comparing between text of the same language, or comparing between different languages where the direction of translation is unknown or indirect</rdfs:comment>
        <rdfs:label xml:lang="en">is close rendering of</rdfs:label>
        <rdfs:seeAlso xml:lang="en">isLooseRenderingOf</rdfs:seeAlso>
    </owl:ObjectProperty>
    


    <!-- http://purl.org/saws/ontology#isCloseTranslationOf -->

    <owl:ObjectProperty rdf:about="http://purl.org/saws/ontology#isCloseTranslationOf">
        <rdfs:subPropertyOf rdf:resource="http://purl.org/saws/ontology#isDirectTranslationOf"/>
        <rdf:type rdf:resource="http://www.w3.org/2002/07/owl#AsymmetricProperty"/>
        <rdfs:domain rdf:resource="http://erlangen-crm.org/current/E33_Linguistic_Object"/>
        <rdfs:range rdf:resource="http://erlangen-crm.org/current/E33_Linguistic_Object"/>
        <rdfs:comment xml:lang="en">A LinguisticObject is related to another LinguisticObject in that it conveys the same ideas, but is expressed in a different language (FRBRoo: an Expression of the same Work in a different Language). This property indicates that the translated text is a close interpretation of the original text 

For comparing between different languages (where a translation act is known to have taken place directly between those documents, in a particular direction)</rdfs:comment>
        <rdfs:label xml:lang="en">is close translation of</rdfs:label>
        <rdfs:seeAlso xml:lang="en">isLooseTranslationOf
isCloseRenderingOf</rdfs:seeAlso>
    </owl:ObjectProperty>
    


    <!-- http://purl.org/saws/ontology#isCommentOn -->

    <owl:ObjectProperty rdf:about="http://purl.org/saws/ontology#isCommentOn">
        <rdfs:subPropertyOf rdf:resource="http://purl.org/saws/ontology#refersTo"/>
        <rdfs:domain rdf:resource="http://purl.org/saws/ontology#Comment"/>
        <rdfs:range rdf:resource="http://erlangen-crm.org/current/E1_CRM_Entity"/>
        <rdfs:comment xml:lang="en">To indicate that an editorial Comment is being made about something</rdfs:comment>
        <rdfs:label xml:lang="en">is comment on</rdfs:label>
    </owl:ObjectProperty>
    


    <!-- http://purl.org/saws/ontology#isComponentOf -->

    <owl:ObjectProperty rdf:about="http://purl.org/saws/ontology#isComponentOf">
        <rdfs:subPropertyOf rdf:resource="http://erlangen-crm.org/efrbroo/R5i_is_component_of"/>
        <rdfs:domain rdf:resource="http://erlangen-crm.org/efrbroo/F2_Expression"/>
        <rdfs:range rdf:resource="http://erlangen-crm.org/efrbroo/F2_Expression"/>
    </owl:ObjectProperty>
    


    <!-- http://purl.org/saws/ontology#isCopiedBy -->

    <owl:ObjectProperty rdf:about="http://purl.org/saws/ontology#isCopiedBy">
        <rdfs:subPropertyOf rdf:resource="http://purl.org/saws/ontology#isWrittenBy"/>
        <owl:inverseOf rdf:resource="http://purl.org/saws/ontology#isCopierOf"/>
        <rdfs:domain>
            <owl:Class>
                <owl:intersectionOf rdf:parseType="Collection">
                    <rdf:Description rdf:about="http://erlangen-crm.org/current/E33_Linguistic_Object"/>
                    <owl:Class>
                        <owl:complementOf rdf:resource="http://purl.org/saws/ontology#Edition"/>
                    </owl:Class>
                </owl:intersectionOf>
            </owl:Class>
        </rdfs:domain>
        <rdfs:range rdf:resource="http://purl.org/saws/ontology#Scribe"/>
        <rdfs:comment xml:lang="en">A LinguisticObject (except Edition) is copied by this Scribe</rdfs:comment>
        <rdfs:label xml:lang="en">is copied by</rdfs:label>
    </owl:ObjectProperty>
    


    <!-- http://purl.org/saws/ontology#isCopierOf -->

    <owl:ObjectProperty rdf:about="http://purl.org/saws/ontology#isCopierOf">
        <rdfs:subPropertyOf rdf:resource="http://purl.org/saws/ontology#hasWritten"/>
        <rdfs:domain rdf:resource="http://purl.org/saws/ontology#Scribe"/>
        <rdfs:range>
            <owl:Class>
                <owl:intersectionOf rdf:parseType="Collection">
                    <rdf:Description rdf:about="http://erlangen-crm.org/current/E33_Linguistic_Object"/>
                    <owl:Class>
                        <owl:complementOf rdf:resource="http://purl.org/saws/ontology#Edition"/>
                    </owl:Class>
                </owl:intersectionOf>
            </owl:Class>
        </rdfs:range>
        <rdfs:comment xml:lang="en">A Scribe has written or copied this LinguisticObject (any Linguistic Object except Edition)</rdfs:comment>
        <rdfs:label xml:lang="en">is copier of</rdfs:label>
    </owl:ObjectProperty>
    


    <!-- http://purl.org/saws/ontology#isDescendantOf -->

    <owl:ObjectProperty rdf:about="http://purl.org/saws/ontology#isDescendantOf">
        <rdfs:subPropertyOf rdf:resource="http://purl.org/saws/ontology#isInSameFamilyAs"/>
        <rdf:type rdf:resource="http://www.w3.org/2002/07/owl#TransitiveProperty"/>
        <owl:propertyChainAxiom rdf:parseType="Collection">
            <rdf:Description rdf:about="http://purl.org/saws/ontology#isChildOf"/>
            <rdf:Description rdf:about="http://purl.org/saws/ontology#isDescendantOf"/>
        </owl:propertyChainAxiom>
        <rdfs:comment xml:lang="en">An ancestor OriginalMaterial is a source material (direct or indirect) for the production of part or all of the descendant OriginalMaterial</rdfs:comment>
        <rdfs:label xml:lang="en">is descendant of</rdfs:label>
    </owl:ObjectProperty>
    


    <!-- http://purl.org/saws/ontology#isDifferentTo -->

    <owl:ObjectProperty rdf:about="http://purl.org/saws/ontology#isDifferentTo">
        <rdf:type rdf:resource="http://www.w3.org/2002/07/owl#SymmetricProperty"/>
        <rdfs:comment xml:lang="en">To explicitly say that two things are different from each other</rdfs:comment>
        <rdfs:label xml:lang="en">is different to</rdfs:label>
    </owl:ObjectProperty>
    


    <!-- http://purl.org/saws/ontology#isDirectCopyOf -->

    <owl:ObjectProperty rdf:about="http://purl.org/saws/ontology#isDirectCopyOf">
        <rdfs:subPropertyOf rdf:resource="http://erlangen-crm.org/current/P130_shows_features_of"/>
        <rdfs:domain rdf:resource="http://erlangen-crm.org/current/E33_Linguistic_Object"/>
        <rdfs:range rdf:resource="http://erlangen-crm.org/current/E33_Linguistic_Object"/>
    </owl:ObjectProperty>
    


    <!-- http://purl.org/saws/ontology#isDirectTranslationOf -->

    <owl:ObjectProperty rdf:about="http://purl.org/saws/ontology#isDirectTranslationOf">
        <rdfs:subPropertyOf rdf:resource="http://erlangen-crm.org/current/P73_has_translation"/>
        <rdf:type rdf:resource="http://www.w3.org/2002/07/owl#AsymmetricProperty"/>
        <rdfs:domain rdf:resource="http://erlangen-crm.org/current/E33_Linguistic_Object"/>
        <rdfs:range rdf:resource="http://erlangen-crm.org/current/E33_Linguistic_Object"/>
        <owl:propertyDisjointWith rdf:resource="http://purl.org/saws/ontology#isIndirectTranslationOf"/>
        <rdfs:comment xml:lang="en">To indicate that the translator worked directly from an MS or text which we have identified, to produce the target linguistic object. A LinguisticObject is related to another LinguisticObject in that it conveys the same ideas (FRBRoo: Work), but is expressed in a different language (FRBRoo: a different and longer Expression).

For comparing between different languages (where a translation act is known to have taken place directly between those documents, in a particular direction)</rdfs:comment>
        <rdfs:label xml:lang="en">is direct translation of</rdfs:label>
        <rdfs:seeAlso xml:lang="en">isIndirectTranslationOf
isTransliterationOf</rdfs:seeAlso>
    </owl:ObjectProperty>
    


    <!-- http://purl.org/saws/ontology#isEditedBy -->

    <owl:ObjectProperty rdf:about="http://purl.org/saws/ontology#isEditedBy">
        <rdfs:subPropertyOf rdf:resource="http://purl.org/saws/ontology#isWrittenBy"/>
        <owl:inverseOf rdf:resource="http://purl.org/saws/ontology#isEditorOf"/>
        <rdfs:domain rdf:resource="http://purl.org/saws/ontology#Edition"/>
        <rdfs:range rdf:resource="http://purl.org/saws/ontology#Editor"/>
        <rdfs:comment xml:lang="en">An Edition is edited by an Editor (someone from the SAWS team or another modern-day scholar)</rdfs:comment>
        <rdfs:label xml:lang="en">is edited by</rdfs:label>
    </owl:ObjectProperty>
    


    <!-- http://purl.org/saws/ontology#isEditorOf -->

    <owl:ObjectProperty rdf:about="http://purl.org/saws/ontology#isEditorOf">
        <rdfs:subPropertyOf rdf:resource="http://purl.org/saws/ontology#hasWritten"/>
        <rdfs:domain rdf:resource="http://purl.org/saws/ontology#Editor"/>
        <rdfs:range rdf:resource="http://purl.org/saws/ontology#Edition"/>
        <rdfs:comment xml:lang="en">An Editor (a modern-day scholar, e.g. someone from the SAWS team) has edited an Edition</rdfs:comment>
        <rdfs:label xml:lang="en">is editor of</rdfs:label>
    </owl:ObjectProperty>
    


    <!-- http://purl.org/saws/ontology#isFromSamePlaceAs -->

    <owl:ObjectProperty rdf:about="http://purl.org/saws/ontology#isFromSamePlaceAs">
        <rdfs:subPropertyOf rdf:resource="http://purl.org/saws/ontology#isRelatedTo"/>
        <rdf:type rdf:resource="http://www.w3.org/2002/07/owl#SymmetricProperty"/>
        <rdf:type rdf:resource="http://www.w3.org/2002/07/owl#TransitiveProperty"/>
        <rdfs:domain>
            <owl:Class>
                <owl:unionOf rdf:parseType="Collection">
                    <rdf:Description rdf:about="http://purl.org/saws/ontology#ManuscriptPart"/>
                    <rdf:Description rdf:about="http://purl.org/saws/ontology#PhysicalManuscript"/>
                    <rdf:Description rdf:about="http://purl.org/saws/ontology#ReconstructedManuscript"/>
                </owl:unionOf>
            </owl:Class>
        </rdfs:domain>
        <rdfs:range>
            <owl:Class>
                <owl:unionOf rdf:parseType="Collection">
                    <rdf:Description rdf:about="http://purl.org/saws/ontology#ManuscriptPart"/>
                    <rdf:Description rdf:about="http://purl.org/saws/ontology#PhysicalManuscript"/>
                    <rdf:Description rdf:about="http://purl.org/saws/ontology#ReconstructedManuscript"/>
                </owl:unionOf>
            </owl:Class>
        </rdfs:range>
        <owl:propertyChainAxiom rdf:parseType="Collection">
            <rdf:Description rdf:about="http://purl.org/saws/ontology#isWrittenAt"/>
            <rdf:Description rdf:about="http://purl.org/saws/ontology#isLocationForWritingOf"/>
        </owl:propertyChainAxiom>
        <rdfs:comment xml:lang="en">The two manuscripts (or parts of the manuscripts) have been copied/produced in the same Place/Institution</rdfs:comment>
        <rdfs:label xml:lang="en">is from same place as</rdfs:label>
        <rdfs:seeAlso xml:lang="en">(Place or Institution) isLocationForWritingOf Material
Material isWrittenAt (Place or Institution)

PhysicalManuscript/ReconstructedManuscript/ManuscriptPart isBySameScribeAs  PhysicalManuscript/ReconstructedManuscriptPart</rdfs:seeAlso>
    </owl:ObjectProperty>
    


    <!-- http://purl.org/saws/ontology#isIdentifiedBy -->

    <owl:ObjectProperty rdf:about="http://purl.org/saws/ontology#isIdentifiedBy">
        <rdfs:subPropertyOf rdf:resource="http://erlangen-crm.org/current/P94i_was_created_by"/>
        <rdfs:domain>
            <owl:Class>
                <owl:unionOf rdf:parseType="Collection">
                    <rdf:Description rdf:about="http://purl.org/saws/ontology#Editor"/>
                    <rdf:Description rdf:about="http://purl.org/saws/ontology#Scribe"/>
                </owl:unionOf>
            </owl:Class>
        </rdfs:domain>
        <rdfs:range>
            <owl:Class>
                <owl:unionOf rdf:parseType="Collection">
                    <rdf:Description rdf:about="http://purl.org/saws/ontology#EditorSection"/>
                    <rdf:Description rdf:about="http://purl.org/saws/ontology#ScribeSection"/>
                </owl:unionOf>
            </owl:Class>
        </rdfs:range>
    </owl:ObjectProperty>
    


    <!-- http://purl.org/saws/ontology#isInLanguage -->

    <owl:ObjectProperty rdf:about="http://purl.org/saws/ontology#isInLanguage">
        <rdfs:subPropertyOf rdf:resource="http://erlangen-crm.org/current/P72_has_language"/>
        <rdfs:domain rdf:resource="http://erlangen-crm.org/current/E33_Linguistic_Object"/>
        <rdfs:range rdf:resource="http://erlangen-crm.org/current/E56_Language"/>
        <rdfs:comment xml:lang="en">A LinguisticObject is text in the specified Language</rdfs:comment>
        <rdfs:label xml:lang="en">is in language</rdfs:label>
    </owl:ObjectProperty>
    


    <!-- http://purl.org/saws/ontology#isInSameFamilyAs -->

    <owl:ObjectProperty rdf:about="http://purl.org/saws/ontology#isInSameFamilyAs">
        <rdfs:subPropertyOf rdf:resource="http://purl.org/saws/ontology#isRelatedTo"/>
        <rdf:type rdf:resource="http://www.w3.org/2002/07/owl#SymmetricProperty"/>
        <rdf:type rdf:resource="http://www.w3.org/2002/07/owl#TransitiveProperty"/>
        <rdfs:domain rdf:resource="http://purl.org/saws/ontology#OriginalMaterial"/>
        <rdfs:range rdf:resource="http://purl.org/saws/ontology#OriginalMaterial"/>
        <owl:propertyChainAxiom rdf:parseType="Collection">
            <rdf:Description rdf:about="http://purl.org/saws/ontology#isMemberOf"/>
            <rdf:Description rdf:about="http://purl.org/saws/ontology#hasMember"/>
        </owl:propertyChainAxiom>
        <rdfs:comment xml:lang="en">Two OriginalMaterials are related by being part of the same Family of Original Materials</rdfs:comment>
        <rdfs:label xml:lang="en">is in same family as</rdfs:label>
    </owl:ObjectProperty>
    


    <!-- http://purl.org/saws/ontology#isIndirectTranslationOf -->

    <owl:ObjectProperty rdf:about="http://purl.org/saws/ontology#isIndirectTranslationOf">
        <rdfs:subPropertyOf rdf:resource="http://purl.org/saws/ontology#isVariantOf"/>
        <rdfs:domain rdf:resource="http://erlangen-crm.org/current/E33_Linguistic_Object"/>
        <rdfs:range rdf:resource="http://erlangen-crm.org/current/E33_Linguistic_Object"/>
        <rdfs:comment xml:lang="en">To indicate where the Scribe worked from a lost translation/version or series of translations/versions to produce the target LinguisticObject. This relation should be used when we know that one LinguisticObject is a source of another (in a different language) and we want to assert that one text is not a direct translation from a previous document but where other unknown documents were involved in the process of going from one to another.

For comparing between text of the same language, or comparing between different languages where the direction of translation is unknown or indirect</rdfs:comment>
        <rdfs:label xml:lang="en">is indirect translation of</rdfs:label>
        <rdfs:seeAlso xml:lang="en">isDirectTranslationOf</rdfs:seeAlso>
    </owl:ObjectProperty>
    


    <!-- http://purl.org/saws/ontology#isLocatedAt -->

    <owl:ObjectProperty rdf:about="http://purl.org/saws/ontology#isLocatedAt">
        <rdfs:subPropertyOf rdf:resource="http://erlangen-crm.org/current/P53_has_former_or_current_location"/>
        <rdfs:subPropertyOf rdf:resource="http://purl.org/saws/ontology#isRelatedTo"/>
        <owl:inverseOf rdf:resource="http://purl.org/saws/ontology#isLocationOf"/>
        <rdf:type rdf:resource="http://www.w3.org/2002/07/owl#TransitiveProperty"/>
        <rdfs:domain rdf:resource="http://erlangen-crm.org/current/E18_Physical_Thing"/>
        <rdfs:range rdf:resource="http://erlangen-crm.org/current/E53_Place"/>
        <rdfs:comment xml:lang="en">A physical thing is (or was) located at a particular location (Place or Locus)

NB Use this relation if you are talking about a physically-existing object being located at a physical place. Use physicallyLocatedAt if you are talking about an abstract linguistic object being found at a particular locus.</rdfs:comment>
        <rdfs:label xml:lang="en">is located at</rdfs:label>
        <rdfs:seeAlso xml:lang="en">physicallyLocatedAt</rdfs:seeAlso>
    </owl:ObjectProperty>
    


    <!-- http://purl.org/saws/ontology#isLocationForWritingOf -->

    <owl:ObjectProperty rdf:about="http://purl.org/saws/ontology#isLocationForWritingOf">
        <rdfs:subPropertyOf rdf:resource="http://purl.org/saws/ontology#isRelatedTo"/>
        <owl:inverseOf rdf:resource="http://purl.org/saws/ontology#isWrittenAt"/>
        <rdfs:domain>
            <owl:Class>
                <owl:unionOf rdf:parseType="Collection">
                    <rdf:Description rdf:about="http://erlangen-crm.org/current/E53_Place"/>
                    <rdf:Description rdf:about="http://purl.org/saws/ontology#Institution"/>
                </owl:unionOf>
            </owl:Class>
        </rdfs:domain>
        <rdfs:range rdf:resource="http://erlangen-crm.org/current/E33_Linguistic_Object"/>
        <rdfs:comment xml:lang="en">A Place is the location witnessing the writing (or transcription) of a LinguisticObject</rdfs:comment>
        <rdfs:label xml:lang="en">is location for writing of</rdfs:label>
        <rdfs:seeAlso xml:lang="en">isLocationOf</rdfs:seeAlso>
    </owl:ObjectProperty>
    


    <!-- http://purl.org/saws/ontology#isLocationOf -->

    <owl:ObjectProperty rdf:about="http://purl.org/saws/ontology#isLocationOf">
        <rdfs:subPropertyOf rdf:resource="http://erlangen-crm.org/current/P53i_is_former_or_current_location_of"/>
        <rdfs:subPropertyOf rdf:resource="http://purl.org/saws/ontology#isRelatedTo"/>
        <rdf:type rdf:resource="http://www.w3.org/2002/07/owl#TransitiveProperty"/>
        <rdfs:domain rdf:resource="http://erlangen-crm.org/current/E53_Place"/>
        <rdfs:range rdf:resource="http://erlangen-crm.org/current/E18_Physical_Thing"/>
        <rdfs:comment xml:lang="en">A particular Place or Locus is (or was) the location of a physical thing.

NB Use this relation if you are talking about the physical location of a physically-existing object. Use physicalLocationOf if you are talking about the physical location for an abstract linguistic object.</rdfs:comment>
        <rdfs:label xml:lang="en">is location of</rdfs:label>
        <rdfs:seeAlso xml:lang="en">physicalLocationOf</rdfs:seeAlso>
    </owl:ObjectProperty>
    


    <!-- http://purl.org/saws/ontology#isLongerTranslationOf -->

    <owl:ObjectProperty rdf:about="http://purl.org/saws/ontology#isLongerTranslationOf">
        <rdfs:subPropertyOf rdf:resource="http://purl.org/saws/ontology#isDirectTranslationOf"/>
        <owl:inverseOf rdf:resource="http://purl.org/saws/ontology#isShorterTranslationOf"/>
        <rdf:type rdf:resource="http://www.w3.org/2002/07/owl#AsymmetricProperty"/>
        <rdfs:domain rdf:resource="http://erlangen-crm.org/current/E33_Linguistic_Object"/>
        <rdfs:range rdf:resource="http://erlangen-crm.org/current/E33_Linguistic_Object"/>
        <rdfs:comment xml:lang="en">A LinguisticObject is an enhanced or expanded copy of another LinguisticObject.

For comparing between different languages (where a translation act is known to have taken place directly between those documents, in a particular direction)</rdfs:comment>
        <rdfs:label xml:lang="en">is longer translation of</rdfs:label>
        <rdfs:seeAlso xml:lang="en">isLongerVersionOf</rdfs:seeAlso>
    </owl:ObjectProperty>
    


    <!-- http://purl.org/saws/ontology#isLongerVersionOf -->

    <owl:ObjectProperty rdf:about="http://purl.org/saws/ontology#isLongerVersionOf">
        <rdfs:subPropertyOf rdf:resource="http://purl.org/saws/ontology#isVersionOf"/>
        <owl:inverseOf rdf:resource="http://purl.org/saws/ontology#isShorterVersionOf"/>
        <rdfs:domain rdf:resource="http://erlangen-crm.org/current/E33_Linguistic_Object"/>
        <rdfs:range rdf:resource="http://erlangen-crm.org/current/E33_Linguistic_Object"/>
        <rdfs:comment xml:lang="en">A LinguisticObject is related to another LinguisticObject in that it conveys the same ideas (FRBRoo: Work), but is expressed in a longer version (FRBRoo: a different and longer Expression) which is an extension of the original text in some way. 

For comparing between text of the same language, or comparing between different languages where the direction of translation is unknown or indirect</rdfs:comment>
        <rdfs:label xml:lang="en">is longer version of</rdfs:label>
    </owl:ObjectProperty>
    


    <!-- http://purl.org/saws/ontology#isLooseRenderingOf -->

    <owl:ObjectProperty rdf:about="http://purl.org/saws/ontology#isLooseRenderingOf">
        <rdfs:subPropertyOf rdf:resource="http://purl.org/saws/ontology#isVariantOf"/>
        <rdfs:domain rdf:resource="http://erlangen-crm.org/current/E33_Linguistic_Object"/>
        <rdfs:range rdf:resource="http://erlangen-crm.org/current/E33_Linguistic_Object"/>
        <rdfs:comment xml:lang="en">From one dialect or genre into another. This property specifies the source and target LinguisticObject involved (respectively) when rendering one LinguisticObject instance to express it in a related but different way (not necessarily in a different Language), resulting in a new LinguisticObject e.g. poetry into prose, or from one dialect to another, or a paraphrase being made. This property indicates that the new LinguisticObject is a loose rendering of the original LinguisticObject

For comparing between text of the same language, or comparing between different languages where the direction of translation is unknown or indirect</rdfs:comment>
        <rdfs:label xml:lang="en">is loose rendering of</rdfs:label>
        <rdfs:seeAlso xml:lang="en">isCloseRenderingOf</rdfs:seeAlso>
    </owl:ObjectProperty>
    


    <!-- http://purl.org/saws/ontology#isLooseTranslationOf -->

    <owl:ObjectProperty rdf:about="http://purl.org/saws/ontology#isLooseTranslationOf">
        <rdfs:subPropertyOf rdf:resource="http://purl.org/saws/ontology#isDirectTranslationOf"/>
        <rdf:type rdf:resource="http://www.w3.org/2002/07/owl#AsymmetricProperty"/>
        <rdfs:domain rdf:resource="http://erlangen-crm.org/current/E33_Linguistic_Object"/>
        <rdfs:range rdf:resource="http://erlangen-crm.org/current/E33_Linguistic_Object"/>
        <rdfs:comment xml:lang="en">A LinguisticObject is related to another LinguisticObject in that it conveys the same ideas (FRBRoo: Work), but is expressed in a different language (FRBRoo: a different and longer Expression). This property indicates that the translated text is a loose interpretation of the original text

For comparing between different languages (where a translation act is known to have taken place directly between those documents, in a particular direction)</rdfs:comment>
        <rdfs:label xml:lang="en">is loose translation of</rdfs:label>
        <rdfs:seeAlso xml:lang="en">isCloseTranslationOf
isLooseRenderingOf</rdfs:seeAlso>
    </owl:ObjectProperty>
    


    <!-- http://purl.org/saws/ontology#isMemberOf -->

    <owl:ObjectProperty rdf:about="http://purl.org/saws/ontology#isMemberOf">
        <rdfs:subPropertyOf rdf:resource="http://purl.org/saws/ontology#isRelatedTo"/>
        <rdf:type rdf:resource="http://www.w3.org/2002/07/owl#TransitiveProperty"/>
        <rdf:type rdf:resource="http://www.w3.org/2002/07/owl#ReflexiveProperty"/>
        <rdfs:domain rdf:resource="http://erlangen-crm.org/current/E1_CRM_Entity"/>
        <rdfs:range rdf:resource="http://erlangen-crm.org/current/E1_CRM_Entity"/>
        <rdfs:comment xml:lang="en">We use isMemberOf to indicate:
- An OriginalMaterial is member of a Family of related
OriginalMaterials
- A Person is member of an Institution</rdfs:comment>
        <rdfs:label xml:lang="en">is member of</rdfs:label>
        <rdfs:seeAlso xml:lang="en">dct:isPartOf
efrbroo:R10i_is_member_of
ecrm:P107i_is_current_or_former_member_of</rdfs:seeAlso>
    </owl:ObjectProperty>
    


    <!-- http://purl.org/saws/ontology#isNotPresentIn -->

    <owl:ObjectProperty rdf:about="http://purl.org/saws/ontology#isNotPresentIn">
        <rdfs:domain rdf:resource="http://erlangen-crm.org/current/E33_Linguistic_Object"/>
        <rdfs:range rdf:resource="http://erlangen-crm.org/current/E33_Linguistic_Object"/>
        <rdfs:comment xml:lang="en">To specify that a piece of text is missing from a LinguisticObject, for example if this text appears in a corresponding part of a manuscript from the same Family</rdfs:comment>
        <rdfs:label xml:lang="en">is not present in</rdfs:label>
    </owl:ObjectProperty>
    


    <!-- http://purl.org/saws/ontology#isOlderThan -->

    <owl:ObjectProperty rdf:about="http://purl.org/saws/ontology#isOlderThan">
        <rdfs:subPropertyOf rdf:resource="http://purl.org/saws/ontology#isRelatedTo"/>
        <owl:inverseOf rdf:resource="http://purl.org/saws/ontology#isYoungerThan"/>
        <rdfs:domain rdf:resource="http://erlangen-crm.org/current/E24_Physical_Man-Made_Thing"/>
        <rdfs:range rdf:resource="http://erlangen-crm.org/current/E24_Physical_Man-Made_Thing"/>
        <owl:propertyChainAxiom rdf:parseType="Collection">
            <rdf:Description rdf:about="http://erlangen-crm.org/current/P108i_was_produced_by"/>
            <rdf:Description rdf:about="http://erlangen-crm.org/current/P120_occurs_before"/>
            <rdf:Description rdf:about="http://erlangen-crm.org/current/P108_has_produced"/>
        </owl:propertyChainAxiom>
        <rdfs:comment xml:lang="en">A Physical man-made thing (physical manuscript) is older than (i.e. was produced earlier in time than) another specified Physical man-made thing</rdfs:comment>
        <rdfs:label xml:lang="en">is older than</rdfs:label>
    </owl:ObjectProperty>
    


    <!-- http://purl.org/saws/ontology#isParentOf -->

    <owl:ObjectProperty rdf:about="http://purl.org/saws/ontology#isParentOf">
        <rdfs:subPropertyOf rdf:resource="http://purl.org/saws/ontology#isAncestorOf"/>
        <rdfs:comment xml:lang="en">The parent OriginalMaterial is a direct source for the production of part or all of the child OriginalMaterial</rdfs:comment>
        <rdfs:label xml:lang="en">is parent of</rdfs:label>
    </owl:ObjectProperty>
    


    <!-- http://purl.org/saws/ontology#isReferencedBy -->

    <owl:ObjectProperty rdf:about="http://purl.org/saws/ontology#isReferencedBy">
        <rdfs:subPropertyOf rdf:resource="http://erlangen-crm.org/current/P67i_is_referred_to_by"/>
        <rdfs:subPropertyOf rdf:resource="http://purl.org/saws/ontology#isRelatedTo"/>
        <owl:inverseOf rdf:resource="http://purl.org/saws/ontology#refersTo"/>
        <rdfs:domain rdf:resource="http://erlangen-crm.org/current/E1_CRM_Entity"/>
        <rdfs:range rdf:resource="http://erlangen-crm.org/current/E33_Linguistic_Object"/>
        <rdfs:comment xml:lang="en">This property allows you to say that an object or some text (internal to that document or from an external source) is referred to in the text of a LinguisticObject, e.g. by being described or being alluded to</rdfs:comment>
        <rdfs:label xml:lang="en">is referenced by</rdfs:label>
    </owl:ObjectProperty>
    


    <!-- http://purl.org/saws/ontology#isRelatedTo -->

    <owl:ObjectProperty rdf:about="http://purl.org/saws/ontology#isRelatedTo">
        <rdf:type rdf:resource="http://www.w3.org/2002/07/owl#SymmetricProperty"/>
        <rdfs:domain rdf:resource="http://erlangen-crm.org/current/E33_Linguistic_Object"/>
        <rdfs:range rdf:resource="http://erlangen-crm.org/current/E33_Linguistic_Object"/>
        <rdfs:comment xml:lang="en">Two things are related in some way. This relation may be used
where the details of the link are to be refined at a later date, or where some relation is seen but the annotater cannot be more specific than to indicate that this relationship exists.</rdfs:comment>
        <rdfs:label xml:lang="en">is related to</rdfs:label>
    </owl:ObjectProperty>
    


    <!-- http://purl.org/saws/ontology#isSequentiallySameAs -->

    <owl:ObjectProperty rdf:about="http://purl.org/saws/ontology#isSequentiallySameAs">
        <rdfs:subPropertyOf rdf:resource="http://purl.org/saws/ontology#isRelatedTo"/>
        <rdf:type rdf:resource="http://www.w3.org/2002/07/owl#SymmetricProperty"/>
        <rdf:type rdf:resource="http://www.w3.org/2002/07/owl#TransitiveProperty"/>
        <rdfs:domain>
            <owl:Class>
                <owl:unionOf rdf:parseType="Collection">
                    <rdf:Description rdf:about="http://purl.org/saws/ontology#CollectionInstance"/>
                    <rdf:Description rdf:about="http://purl.org/saws/ontology#Section"/>
                </owl:unionOf>
            </owl:Class>
        </rdfs:domain>
        <rdfs:range>
            <owl:Class>
                <owl:unionOf rdf:parseType="Collection">
                    <rdf:Description rdf:about="http://purl.org/saws/ontology#CollectionInstance"/>
                    <rdf:Description rdf:about="http://purl.org/saws/ontology#Section"/>
                </owl:unionOf>
            </owl:Class>
        </rdfs:range>
        <rdfs:comment xml:lang="en">A CollectionInstance or Section has the same sequential structure as another CollectionInstance or Section. N.B. CollectionInstances contain sequences of ordered Sections. Sections contain sequences of ordered ContentItems</rdfs:comment>
        <rdfs:label xml:lang="en">is sequentially same as</rdfs:label>
        <rdfs:seeAlso xml:lang="en">isSequentiallySimilarTo
isSubSequenceOf</rdfs:seeAlso>
    </owl:ObjectProperty>
    


    <!-- http://purl.org/saws/ontology#isSequentiallySimilarTo -->

    <owl:ObjectProperty rdf:about="http://purl.org/saws/ontology#isSequentiallySimilarTo">
        <rdfs:subPropertyOf rdf:resource="http://purl.org/saws/ontology#isRelatedTo"/>
        <rdfs:domain>
            <owl:Class>
                <owl:unionOf rdf:parseType="Collection">
                    <rdf:Description rdf:about="http://purl.org/saws/ontology#CollectionInstance"/>
                    <rdf:Description rdf:about="http://purl.org/saws/ontology#Section"/>
                </owl:unionOf>
            </owl:Class>
        </rdfs:domain>
        <rdfs:range>
            <owl:Class>
                <owl:unionOf rdf:parseType="Collection">
                    <rdf:Description rdf:about="http://purl.org/saws/ontology#CollectionInstance"/>
                    <rdf:Description rdf:about="http://purl.org/saws/ontology#Section"/>
                </owl:unionOf>
            </owl:Class>
        </rdfs:range>
        <rdfs:comment xml:lang="en">A CollectionInstance or Section has a slightly different but related sequential structure to another CollectionInstance or Section. N.B. CollectionInstances contain sequences of ordered Sections. Sections contain sequences of ordered ContentItems</rdfs:comment>
        <rdfs:label xml:lang="en">is sequentially similar to</rdfs:label>
        <rdfs:seeAlso xml:lang="en">isSequentiallySameAs
isSubSequenceOf</rdfs:seeAlso>
    </owl:ObjectProperty>
    


    <!-- http://purl.org/saws/ontology#isShorterTranslationOf -->

    <owl:ObjectProperty rdf:about="http://purl.org/saws/ontology#isShorterTranslationOf">
        <rdfs:subPropertyOf rdf:resource="http://purl.org/saws/ontology#isDirectTranslationOf"/>
        <rdf:type rdf:resource="http://www.w3.org/2002/07/owl#AsymmetricProperty"/>
        <rdfs:domain rdf:resource="http://erlangen-crm.org/current/E33_Linguistic_Object"/>
        <rdfs:range rdf:resource="http://erlangen-crm.org/current/E33_Linguistic_Object"/>
        <owl:propertyDisjointWith rdf:resource="http://purl.org/saws/ontology#isShorterVersionOf"/>
        <rdfs:comment xml:lang="en">A LinguisticObject is a condensed copy of another LinguisticObject.

For comparing between different languages (where a translation act is known to have taken place directly between those documents, in a particular direction)</rdfs:comment>
        <rdfs:label xml:lang="en">is shorter translation of</rdfs:label>
        <rdfs:seeAlso xml:lang="en">isShorterVersionOf</rdfs:seeAlso>
    </owl:ObjectProperty>
    


    <!-- http://purl.org/saws/ontology#isShorterVersionOf -->

    <owl:ObjectProperty rdf:about="http://purl.org/saws/ontology#isShorterVersionOf">
        <rdfs:subPropertyOf rdf:resource="http://purl.org/saws/ontology#isVersionOf"/>
        <rdfs:domain rdf:resource="http://erlangen-crm.org/current/E33_Linguistic_Object"/>
        <rdfs:range rdf:resource="http://erlangen-crm.org/current/E33_Linguistic_Object"/>
        <rdfs:comment xml:lang="en">A LinguisticObject is related to another LinguisticObject in that it conveys the same ideas (FRBRoo: Work), but is expressed in a more concise version (FRBRoo: a different and shorter Expression)

For comparing between text of the same language, or comparing between different languages where the direction of translation is unknown or indirect</rdfs:comment>
        <rdfs:label xml:lang="en">is shorter version of</rdfs:label>
        <rdfs:seeAlso xml:lang="en">isShorterTranslationOf</rdfs:seeAlso>
    </owl:ObjectProperty>
    


    <!-- http://purl.org/saws/ontology#isSiblingOf -->

    <owl:ObjectProperty rdf:about="http://purl.org/saws/ontology#isSiblingOf">
        <rdfs:subPropertyOf rdf:resource="http://purl.org/saws/ontology#isInSameFamilyAs"/>
        <rdf:type rdf:resource="http://www.w3.org/2002/07/owl#SymmetricProperty"/>
        <rdfs:comment xml:lang="en">The two OriginalMaterials are produced using the same source(s) OriginalMaterial(s) (as indirect or direct source)</rdfs:comment>
    </owl:ObjectProperty>
    


    <!-- http://purl.org/saws/ontology#isSourceFor -->

    <owl:ObjectProperty rdf:about="http://purl.org/saws/ontology#isSourceFor">
        <rdfs:subPropertyOf rdf:resource="http://purl.org/saws/ontology#isRelatedTo"/>
        <rdfs:domain rdf:resource="http://erlangen-crm.org/current/E33_Linguistic_Object"/>
        <rdfs:range rdf:resource="http://purl.org/saws/ontology#Edition"/>
        <rdfs:comment xml:lang="en">A textual material (manuscripts, collections etc) is one of the source documents on which an edition is based. One &lt;relation&gt; per each textual material)</rdfs:comment>
        <rdfs:label xml:lang="en">is source for</rdfs:label>
    </owl:ObjectProperty>
    


    <!-- http://purl.org/saws/ontology#isSubSequenceOf -->

    <owl:ObjectProperty rdf:about="http://purl.org/saws/ontology#isSubSequenceOf">
        <rdfs:subPropertyOf rdf:resource="http://purl.org/saws/ontology#isRelatedTo"/>
        <rdfs:domain rdf:resource="http://purl.org/saws/ontology#Section"/>
        <rdfs:range rdf:resource="http://purl.org/saws/ontology#Section"/>
        <rdfs:comment xml:lang="en">A Section is formed of a sequence of ContentItems that is a subsequence of the sequence of ContentItems in another Section</rdfs:comment>
        <rdfs:label xml:lang="en">is sub sequence of</rdfs:label>
        <rdfs:seeAlso xml:lang="en">isSequentiallySameAs
isSequentiallySimilarTo</rdfs:seeAlso>
    </owl:ObjectProperty>
    


    <!-- http://purl.org/saws/ontology#isTransliterationOf -->

    <owl:ObjectProperty rdf:about="http://purl.org/saws/ontology#isTransliterationOf">
        <rdfs:subPropertyOf rdf:resource="http://purl.org/saws/ontology#isDirectTranslationOf"/>
        <rdf:type rdf:resource="http://www.w3.org/2002/07/owl#AsymmetricProperty"/>
        <rdfs:domain rdf:resource="http://erlangen-crm.org/current/E33_Linguistic_Object"/>
        <rdfs:range rdf:resource="http://erlangen-crm.org/current/E33_Linguistic_Object"/>
        <rdfs:comment xml:lang="en">A LinguisticObject is a transliteration of another LinguisticObject, i.e. same words but using a different set of characters, e.g. kai isTransliterationOf και </rdfs:comment>
        <rdfs:label xml:lang="en">is transliteration of</rdfs:label>
        <rdfs:seeAlso xml:lang="en">isDirectTranslationOf</rdfs:seeAlso>
    </owl:ObjectProperty>
    


    <!-- http://purl.org/saws/ontology#isTransmittedBy -->

    <owl:ObjectProperty rdf:about="http://purl.org/saws/ontology#isTransmittedBy">
        <rdfs:subPropertyOf rdf:resource="http://purl.org/saws/ontology#isWrittenBy"/>
        <owl:inverseOf rdf:resource="http://purl.org/saws/ontology#isTransmitterOf"/>
        <rdfs:domain>
            <owl:Class>
                <owl:intersectionOf rdf:parseType="Collection">
                    <rdf:Description rdf:about="http://erlangen-crm.org/current/E33_Linguistic_Object"/>
                    <owl:Class>
                        <owl:complementOf rdf:resource="http://purl.org/saws/ontology#Edition"/>
                    </owl:Class>
                </owl:intersectionOf>
            </owl:Class>
        </rdfs:domain>
        <rdfs:range rdf:resource="http://purl.org/saws/ontology#Transmitter"/>
        <rdfs:comment xml:lang="en">A LinguisticObject (except Edition) is transmitted by this Transmitter (Person)</rdfs:comment>
        <rdfs:label xml:lang="en">is transmitted by</rdfs:label>
    </owl:ObjectProperty>
    


    <!-- http://purl.org/saws/ontology#isTransmitterOf -->

    <owl:ObjectProperty rdf:about="http://purl.org/saws/ontology#isTransmitterOf">
        <rdfs:subPropertyOf rdf:resource="http://purl.org/saws/ontology#hasWritten"/>
        <rdfs:domain rdf:resource="http://purl.org/saws/ontology#Transmitter"/>
        <rdfs:range>
            <owl:Class>
                <owl:intersectionOf rdf:parseType="Collection">
                    <rdf:Description rdf:about="http://erlangen-crm.org/current/E33_Linguistic_Object"/>
                    <owl:Class>
                        <owl:complementOf rdf:resource="http://purl.org/saws/ontology#Edition"/>
                    </owl:Class>
                </owl:intersectionOf>
            </owl:Class>
        </rdfs:range>
        <rdfs:comment xml:lang="en">A Transmitter (Person) has transmitted this LinguisticObject (any Linguistic Object except Edition)</rdfs:comment>
        <rdfs:label xml:lang="en">is transmitter of</rdfs:label>
    </owl:ObjectProperty>
    


    <!-- http://purl.org/saws/ontology#isTwinOf -->

    <owl:ObjectProperty rdf:about="http://purl.org/saws/ontology#isTwinOf">
        <rdfs:subPropertyOf rdf:resource="http://purl.org/saws/ontology#isSiblingOf"/>
        <rdf:type rdf:resource="http://www.w3.org/2002/07/owl#SymmetricProperty"/>
        <rdfs:comment xml:lang="en">The two OriginalMaterials are produced using the same direct source(s) OriginalMaterial</rdfs:comment>
        <rdfs:label xml:lang="en">is twin of</rdfs:label>
    </owl:ObjectProperty>
    


    <!-- http://purl.org/saws/ontology#isUnrelatedTo -->

    <owl:ObjectProperty rdf:about="http://purl.org/saws/ontology#isUnrelatedTo">
        <rdf:type rdf:resource="http://www.w3.org/2002/07/owl#SymmetricProperty"/>
        <rdfs:comment xml:lang="en">To explicitly say two things are not at all related but are
completely independent of each other</rdfs:comment>
        <rdfs:label xml:lang="en">is unrelated to</rdfs:label>
    </owl:ObjectProperty>
    


    <!-- http://purl.org/saws/ontology#isVariantOf -->

    <owl:ObjectProperty rdf:about="http://purl.org/saws/ontology#isVariantOf">
        <rdfs:subPropertyOf rdf:resource="http://erlangen-crm.org/current/P130_shows_features_of"/>
        <rdfs:domain rdf:resource="http://erlangen-crm.org/current/E33_Linguistic_Object"/>
        <rdfs:range rdf:resource="http://erlangen-crm.org/current/E33_Linguistic_Object"/>
        <owl:propertyDisjointWith rdf:resource="http://purl.org/saws/ontology#isVariantTranslationOf"/>
        <rdfs:comment xml:lang="en">A LinguisticObject is a variant of another LinguisticObject. NB This property is specialised by its subproperties - this is the default option, but more specialised properties should be used where possible. isVariantOf can be used as a placeholder or temporary annotation in a preliminary stage of annotation

For comparing between text of the same language, or comparing between different languages where the direction of translation is unknown or indirect</rdfs:comment>
        <rdfs:label xml:lang="en">is variant of</rdfs:label>
        <rdfs:seeAlso xml:lang="en">isVariantTranslationOf</rdfs:seeAlso>
    </owl:ObjectProperty>
    


    <!-- http://purl.org/saws/ontology#isVariantTranslationOf -->

    <owl:ObjectProperty rdf:about="http://purl.org/saws/ontology#isVariantTranslationOf">
        <rdfs:subPropertyOf rdf:resource="http://purl.org/saws/ontology#isDirectTranslationOf"/>
        <rdf:type rdf:resource="http://www.w3.org/2002/07/owl#AsymmetricProperty"/>
        <rdfs:domain rdf:resource="http://erlangen-crm.org/current/E33_Linguistic_Object"/>
        <rdfs:range rdf:resource="http://erlangen-crm.org/current/E33_Linguistic_Object"/>
        <rdfs:comment xml:lang="en">A LinguisticObject is a slightly modified copy of another LinguisticObject.

For comparing between different languages (where a translation act is known to have taken place directly between those documents, in a particular direction)</rdfs:comment>
        <rdfs:label xml:lang="en">is variant translation of</rdfs:label>
        <rdfs:seeAlso xml:lang="en">isVariant</rdfs:seeAlso>
    </owl:ObjectProperty>
    


    <!-- http://purl.org/saws/ontology#isVerbatimOf -->

    <owl:ObjectProperty rdf:about="http://purl.org/saws/ontology#isVerbatimOf">
        <rdfs:subPropertyOf rdf:resource="http://purl.org/saws/ontology#isVariantOf"/>
        <rdfs:domain rdf:resource="http://erlangen-crm.org/current/E33_Linguistic_Object"/>
        <rdfs:range rdf:resource="http://erlangen-crm.org/current/E33_Linguistic_Object"/>
        <owl:propertyDisjointWith rdf:resource="http://purl.org/saws/ontology#isVerbatimTranslationOf"/>
        <rdfs:comment xml:lang="en">A LinguisticObject is a verbatim, word-for-word copy of another LinguisticObject.

For comparing between text of the same language, or comparing between different languages where the direction of translation is unknown or indirect</rdfs:comment>
        <rdfs:label xml:lang="en">is verbatim of</rdfs:label>
        <rdfs:seeAlso xml:lang="en">isVerbatimTranslationOf</rdfs:seeAlso>
    </owl:ObjectProperty>
    


    <!-- http://purl.org/saws/ontology#isVerbatimTranslationOf -->

    <owl:ObjectProperty rdf:about="http://purl.org/saws/ontology#isVerbatimTranslationOf">
        <rdfs:subPropertyOf rdf:resource="http://purl.org/saws/ontology#isDirectTranslationOf"/>
        <rdf:type rdf:resource="http://www.w3.org/2002/07/owl#AsymmetricProperty"/>
        <rdfs:domain rdf:resource="http://erlangen-crm.org/current/E33_Linguistic_Object"/>
        <rdfs:comment xml:lang="en">A LinguisticObject is a verbatim, word-for-word copy of another LinguisticObject.

For comparing between different languages (where a translation act is known to have taken place directly between those documents, in a particular direction)</rdfs:comment>
        <rdfs:label xml:lang="en">is verbatim translation of</rdfs:label>
        <rdfs:seeAlso xml:lang="en">isVerbatimOf</rdfs:seeAlso>
    </owl:ObjectProperty>
    


    <!-- http://purl.org/saws/ontology#isVersionInAnotherLanguagOf -->

    <owl:ObjectProperty rdf:about="http://purl.org/saws/ontology#isVersionInAnotherLanguagOf">
        <rdfs:subPropertyOf rdf:resource="http://erlangen-crm.org/current/P130_shows_features_of"/>
        <rdfs:domain rdf:resource="http://erlangen-crm.org/current/E33_Linguistic_Object"/>
        <rdfs:range rdf:resource="http://erlangen-crm.org/current/E33_Linguistic_Object"/>
    </owl:ObjectProperty>
    


    <!-- http://purl.org/saws/ontology#isVersionOf -->

    <owl:ObjectProperty rdf:about="http://purl.org/saws/ontology#isVersionOf">
        <rdfs:subPropertyOf rdf:resource="http://erlangen-crm.org/current/P130_shows_features_of"/>
        <rdfs:domain rdf:resource="http://erlangen-crm.org/current/E33_Linguistic_Object"/>
        <rdfs:range rdf:resource="http://erlangen-crm.org/current/E33_Linguistic_Object"/>
    </owl:ObjectProperty>
    


    <!-- http://purl.org/saws/ontology#isWrittenAt -->

    <owl:ObjectProperty rdf:about="http://purl.org/saws/ontology#isWrittenAt">
        <rdfs:subPropertyOf rdf:resource="http://purl.org/saws/ontology#isRelatedTo"/>
        <rdfs:domain rdf:resource="http://erlangen-crm.org/current/E33_Linguistic_Object"/>
        <rdfs:range>
            <owl:Class>
                <owl:unionOf rdf:parseType="Collection">
                    <rdf:Description rdf:about="http://erlangen-crm.org/current/E53_Place"/>
                    <rdf:Description rdf:about="http://purl.org/saws/ontology#Institution"/>
                </owl:unionOf>
            </owl:Class>
        </rdfs:range>
        <rdfs:comment xml:lang="en">A LinguisticObject is written (or transcribed) at a specified Place</rdfs:comment>
        <rdfs:label xml:lang="en">is written at</rdfs:label>
        <rdfs:seeAlso xml:lang="en">isLocatedAt</rdfs:seeAlso>
    </owl:ObjectProperty>
    


    <!-- http://purl.org/saws/ontology#isWrittenBy -->

    <owl:ObjectProperty rdf:about="http://purl.org/saws/ontology#isWrittenBy">
        <rdfs:subPropertyOf rdf:resource="http://purl.org/saws/ontology#isRelatedTo"/>
        <rdfs:domain rdf:resource="http://erlangen-crm.org/current/E33_Linguistic_Object"/>
        <rdfs:range rdf:resource="http://erlangen-crm.org/current/E21_Person"/>
        <owl:propertyChainAxiom rdf:parseType="Collection">
            <rdf:Description rdf:about="http://erlangen-crm.org/current/P94i_was_created_by"/>
            <rdf:Description rdf:about="http://erlangen-crm.org/current/P14_carried_out_by"/>
        </owl:propertyChainAxiom>
        <rdfs:comment xml:lang="en">A LinguisticObject is written (or transcribed) by a specified Person</rdfs:comment>
        <rdfs:label xml:lang="en">is written by</rdfs:label>
        <rdfs:seeAlso xml:lang="en">Comment commentMadeBy Editor
Marginalia marginaliaAddedBy Scribe</rdfs:seeAlso>
    </owl:ObjectProperty>
    


    <!-- http://purl.org/saws/ontology#isYoungerThan -->

    <owl:ObjectProperty rdf:about="http://purl.org/saws/ontology#isYoungerThan">
        <rdfs:subPropertyOf rdf:resource="http://purl.org/saws/ontology#isRelatedTo"/>
        <rdfs:domain rdf:resource="http://erlangen-crm.org/current/E24_Physical_Man-Made_Thing"/>
        <rdfs:range rdf:resource="http://erlangen-crm.org/current/E24_Physical_Man-Made_Thing"/>
        <owl:propertyChainAxiom rdf:parseType="Collection">
            <rdf:Description rdf:about="http://erlangen-crm.org/current/P108i_was_produced_by"/>
            <rdf:Description rdf:about="http://erlangen-crm.org/current/P120i_occurs_after"/>
            <rdf:Description rdf:about="http://erlangen-crm.org/current/P108_has_produced"/>
        </owl:propertyChainAxiom>
        <rdfs:comment xml:lang="en">A Physical man-made thing (physical manuscript) is younger than (i.e. was produced later in time than) another specified Physical man-made thing</rdfs:comment>
        <rdfs:label xml:lang="en">is younger than</rdfs:label>
    </owl:ObjectProperty>
    


    <!-- http://purl.org/saws/ontology#marginaliaAddedBy -->

    <owl:ObjectProperty rdf:about="http://purl.org/saws/ontology#marginaliaAddedBy">
        <rdfs:subPropertyOf rdf:resource="http://purl.org/saws/ontology#isRelatedTo"/>
        <rdfs:domain rdf:resource="http://purl.org/saws/ontology#Marginalia"/>
        <rdfs:range rdf:resource="http://purl.org/saws/ontology#Scribe"/>
        <owl:propertyChainAxiom rdf:parseType="Collection">
            <rdf:Description rdf:about="http://erlangen-crm.org/current/P94i_was_created_by"/>
            <rdf:Description rdf:about="http://erlangen-crm.org/current/P14_carried_out_by"/>
        </owl:propertyChainAxiom>
        <rdfs:comment xml:lang="en">Marginalia have been physically added onto the manuscript by a Scribe

NB to represent where a comment has been made by a modern-day scholar/editor, not written onto the manuscript, use: Comment commentMadeBy Editor</rdfs:comment>
        <rdfs:label xml:lang="en">marginalia added by</rdfs:label>
        <rdfs:seeAlso xml:lang="en">LinguisticObject isWrittenBy Person
Comment commentMadeBy Editor</rdfs:seeAlso>
    </owl:ObjectProperty>
    


    <!-- http://purl.org/saws/ontology#ownedBy -->

    <owl:ObjectProperty rdf:about="http://purl.org/saws/ontology#ownedBy">
        <rdfs:subPropertyOf rdf:resource="http://purl.org/saws/ontology#isRelatedTo"/>
        <rdfs:domain rdf:resource="http://purl.org/saws/ontology#Material"/>
        <rdfs:range>
            <owl:Class>
                <owl:unionOf rdf:parseType="Collection">
                    <rdf:Description rdf:about="http://erlangen-crm.org/efrbroo/F10_Person"/>
                    <rdf:Description rdf:about="http://purl.org/saws/ontology#Institution"/>
                </owl:unionOf>
            </owl:Class>
        </rdfs:range>
        <owl:propertyChainAxiom rdf:parseType="Collection">
            <rdf:Description rdf:about="http://erlangen-crm.org/current/P128i_is_carried_by"/>
            <rdf:Description rdf:about="http://erlangen-crm.org/current/P51_has_former_or_current_owner"/>
        </owl:propertyChainAxiom>
        <rdfs:comment xml:lang="en">The Material of interest has been owned (in the past or currently) by this particular Person. This would normally be based on a specific statement/mark of ownership.

[nb this will always need a date?]</rdfs:comment>
        <rdfs:label xml:lang="en">owned by</rdfs:label>
    </owl:ObjectProperty>
    


    <!-- http://purl.org/saws/ontology#physicalLocationOf -->

    <owl:ObjectProperty rdf:about="http://purl.org/saws/ontology#physicalLocationOf">
        <rdfs:subPropertyOf rdf:resource="http://purl.org/saws/ontology#isRelatedTo"/>
        <owl:inverseOf rdf:resource="http://purl.org/saws/ontology#physicallyLocatedAt"/>
        <rdfs:domain rdf:resource="http://purl.org/saws/ontology#Locus"/>
        <rdfs:range rdf:resource="http://erlangen-crm.org/current/E33_Linguistic_Object"/>
        <owl:propertyChainAxiom rdf:parseType="Collection">
            <rdf:Description rdf:about="http://purl.org/saws/ontology#isLocationOf"/>
            <rdf:Description rdf:about="http://erlangen-crm.org/efrbroo/R18i_was_created_by"/>
            <rdf:Description rdf:about="http://erlangen-crm.org/efrbroo/R17_created"/>
        </owl:propertyChainAxiom>
        <rdfs:comment xml:lang="en">This lets you describe the physical location of the LinguisticObject, e.g. a particular piece of text, or Marginalia, by recording the Locus that the notes are physically written on in a Material. You can describe the Locus (e.g. folio number, or position on the page) in free text, in as much detail as required, if there is no formal way to describe the location of the text/marginalia] 

NB Use this relation if you are talking about the physical location for an abstract linguistic object. Use isLocationOf if you are talking about the physical location of a physically-existing object.</rdfs:comment>
        <rdfs:label xml:lang="en">physical location of</rdfs:label>
        <rdfs:seeAlso xml:lang="en">isLocationOf</rdfs:seeAlso>
    </owl:ObjectProperty>
    


    <!-- http://purl.org/saws/ontology#physicallyLocatedAt -->

    <owl:ObjectProperty rdf:about="http://purl.org/saws/ontology#physicallyLocatedAt">
        <rdfs:subPropertyOf rdf:resource="http://purl.org/saws/ontology#isRelatedTo"/>
        <rdfs:domain rdf:resource="http://erlangen-crm.org/current/E33_Linguistic_Object"/>
        <rdfs:range rdf:resource="http://purl.org/saws/ontology#Locus"/>
        <owl:propertyChainAxiom rdf:parseType="Collection">
            <rdf:Description rdf:about="http://erlangen-crm.org/efrbroo/R17i_was_created_by"/>
            <rdf:Description rdf:about="http://erlangen-crm.org/efrbroo/R18_created"/>
            <rdf:Description rdf:about="http://purl.org/saws/ontology#isLocatedAt"/>
        </owl:propertyChainAxiom>
        <rdfs:comment xml:lang="en">This lets you describe the physical location of the LinguisticObject, e.g. a particular piece of text, or Marginalia, by recording the Locus that the notes are physically written on in a Material. You can describe the Locus (e.g. folio number, or position on the page) in free text, in as much detail as required, if there is no formal way to describe the location of the text/marginalia

NB Use this relation if you are talking about an abstract linguistic object which is to be found at a particular locus. Use isLocatedAt if you are talking about a physically-existing object being located at a physical place.</rdfs:comment>
        <rdfs:comment xml:lang="en">physically located at</rdfs:comment>
        <rdfs:seeAlso xml:lang="en">isLocatedAt</rdfs:seeAlso>
    </owl:ObjectProperty>
    


    <!-- http://purl.org/saws/ontology#precedes -->

    <owl:ObjectProperty rdf:about="http://purl.org/saws/ontology#precedes">
        <rdfs:subPropertyOf rdf:resource="http://purl.org/saws/ontology#isRelatedTo"/>
        <rdf:type rdf:resource="http://www.w3.org/2002/07/owl#TransitiveProperty"/>
        <rdfs:comment xml:lang="en">A Section/ContentItem/CollectionInstance comes before another Section/ContentItem/CollectionInstance in the document</rdfs:comment>
        <rdfs:label xml:lang="en">precedes</rdfs:label>
    </owl:ObjectProperty>
    


    <!-- http://purl.org/saws/ontology#refersTo -->

    <owl:ObjectProperty rdf:about="http://purl.org/saws/ontology#refersTo">
        <rdfs:subPropertyOf rdf:resource="http://erlangen-crm.org/current/P67_refers_to"/>
        <rdfs:subPropertyOf rdf:resource="http://purl.org/saws/ontology#isRelatedTo"/>
        <rdfs:domain rdf:resource="http://erlangen-crm.org/current/E33_Linguistic_Object"/>
        <rdfs:range rdf:resource="http://erlangen-crm.org/current/E1_CRM_Entity"/>
        <rdfs:comment xml:lang="en">This property allows you to say that the text of a LinguisticObject makes a reference to (or mentions) some other text or object, either within the text (e.g. as allusion) or external to the text (for external things, please give a URI for that object)</rdfs:comment>
        <rdfs:label xml:lang="en">refers to</rdfs:label>
    </owl:ObjectProperty>
    


    <!-- http://purl.org/saws/ontology#usedBy -->

    <owl:ObjectProperty rdf:about="http://purl.org/saws/ontology#usedBy">
        <rdfs:subPropertyOf rdf:resource="http://purl.org/saws/ontology#isRelatedTo"/>
        <rdfs:domain rdf:resource="http://purl.org/saws/ontology#OriginalMaterial"/>
        <rdfs:range rdf:resource="http://erlangen-crm.org/efrbroo/F10_Person"/>
        <owl:propertyChainAxiom rdf:parseType="Collection">
            <rdf:Description rdf:about="http://erlangen-crm.org/current/P16i_was_used_for"/>
            <rdf:Description rdf:about="http://erlangen-crm.org/current/P14_carried_out_by"/>
        </owl:propertyChainAxiom>
        <rdfs:comment xml:lang="en">The Original Material of interest has been used by this particular Person in their work.

[nb this will always need a date?]</rdfs:comment>
        <rdfs:label xml:lang="en">used by</rdfs:label>
    </owl:ObjectProperty>
    


    <!-- 
    ///////////////////////////////////////////////////////////////////////////////////////
    //
    // Classes
    //
    ///////////////////////////////////////////////////////////////////////////////////////
     -->

    


    <!-- http://erlangen-crm.org/current/E18_Physical_Thing -->

    <owl:Class rdf:about="http://erlangen-crm.org/current/E18_Physical_Thing"/>
    


    <!-- http://erlangen-crm.org/current/E1_CRM_Entity -->

    <owl:Class rdf:about="http://erlangen-crm.org/current/E1_CRM_Entity"/>
    


    <!-- http://erlangen-crm.org/current/E21_Person -->

    <owl:Class rdf:about="http://erlangen-crm.org/current/E21_Person">
        <rdfs:comment xml:lang="en">Note for SAWS: this includes any human being, named or otherwise</rdfs:comment>
        <rdfs:label xml:lang="en">person</rdfs:label>
    </owl:Class>
    


    <!-- http://erlangen-crm.org/current/E24_Physical_Man-Made_Thing -->

    <owl:Class rdf:about="http://erlangen-crm.org/current/E24_Physical_Man-Made_Thing"/>
    


    <!-- http://erlangen-crm.org/current/E33_Linguistic_Object -->

    <owl:Class rdf:about="http://erlangen-crm.org/current/E33_Linguistic_Object"/>
    


    <!-- http://erlangen-crm.org/current/E35_Title -->

    <owl:Class rdf:about="http://erlangen-crm.org/current/E35_Title">
        <rdfs:label xml:lang="en">title</rdfs:label>
    </owl:Class>
    


    <!-- http://erlangen-crm.org/current/E36_Visual_Item -->

    <owl:Class rdf:about="http://erlangen-crm.org/current/E36_Visual_Item"/>
    


    <!-- http://erlangen-crm.org/current/E53_Place -->

    <owl:Class rdf:about="http://erlangen-crm.org/current/E53_Place">
        <rdfs:label xml:lang="en">place</rdfs:label>
    </owl:Class>
    


    <!-- http://erlangen-crm.org/current/E56_Language -->

    <owl:Class rdf:about="http://erlangen-crm.org/current/E56_Language">
        <rdfs:comment xml:lang="en">Note for SAWS: This represents language in which a material is written - this is put in the TEI header. 

NB in the TEI header we should use standards for languages, e.g. the more detailed ISO standards at http://www.loc.gov/standards/iso639-2/ , so use “http://id.loc.gov/vocabulary/iso639-2/grc” for Ancient Greek rather than “Greek”</rdfs:comment>
        <rdfs:label xml:lang="en">language</rdfs:label>
    </owl:Class>
    


    <!-- http://erlangen-crm.org/current/E74_Group -->

    <owl:Class rdf:about="http://erlangen-crm.org/current/E74_Group"/>
    


    <!-- http://erlangen-crm.org/efrbroo/F10_Person -->

    <owl:Class rdf:about="http://erlangen-crm.org/efrbroo/F10_Person"/>
    


    <!-- http://erlangen-crm.org/efrbroo/F15_Complex_Work -->

    <owl:Class rdf:about="http://erlangen-crm.org/efrbroo/F15_Complex_Work"/>
    


    <!-- http://erlangen-crm.org/efrbroo/F22_Self-Contained_Expression -->

    <owl:Class rdf:about="http://erlangen-crm.org/efrbroo/F22_Self-Contained_Expression"/>
    


    <!-- http://erlangen-crm.org/efrbroo/F23_Expression_Fragment -->

    <owl:Class rdf:about="http://erlangen-crm.org/efrbroo/F23_Expression_Fragment"/>
    


    <!-- http://erlangen-crm.org/efrbroo/F2_Expression -->

    <owl:Class rdf:about="http://erlangen-crm.org/efrbroo/F2_Expression"/>
    


    <!-- http://erlangen-crm.org/efrbroo/F4_Manifestation_Singleton -->

    <owl:Class rdf:about="http://erlangen-crm.org/efrbroo/F4_Manifestation_Singleton"/>
    


    <!-- http://purl.org/saws/ontology#AbstractManuscriptText -->

    <owl:Class rdf:about="http://purl.org/saws/ontology#AbstractManuscriptText">
        <rdfs:subClassOf rdf:resource="http://purl.org/saws/ontology#OriginalMaterial"/>
        <rdfs:comment xml:lang="en">The text that is written in an manuscript</rdfs:comment>
        <rdfs:label xml:lang="en">abstract manuscript text</rdfs:label>
    </owl:Class>
    


    <!-- http://purl.org/saws/ontology#AttributedAuthor -->

    <owl:Class rdf:about="http://purl.org/saws/ontology#AttributedAuthor">
        <rdfs:subClassOf rdf:resource="http://erlangen-crm.org/current/E21_Person"/>
        <owl:disjointWith rdf:resource="http://purl.org/saws/ontology#Editor"/>
        <rdfs:comment xml:lang="en">Person to whom original authorship of a linguistic object is attributed, as the source of that linguistic object</rdfs:comment>
        <rdfs:label xml:lang="en">attributed author</rdfs:label>
    </owl:Class>
    


    <!-- http://purl.org/saws/ontology#CollectionInstance -->

    <owl:Class rdf:about="http://purl.org/saws/ontology#CollectionInstance">
        <rdfs:subClassOf rdf:resource="http://purl.org/saws/ontology#OriginalMaterial"/>
        <rdfs:comment xml:lang="en">The gnomologium or other compilation/collection on which we are working</rdfs:comment>
        <rdfs:label xml:lang="en">collection instance</rdfs:label>
    </owl:Class>
    


    <!-- http://purl.org/saws/ontology#Comment -->

    <owl:Class rdf:about="http://purl.org/saws/ontology#Comment">
        <rdfs:subClassOf>
            <owl:Class>
                <owl:intersectionOf rdf:parseType="Collection">
                    <rdf:Description rdf:about="http://erlangen-crm.org/current/E33_Linguistic_Object"/>
                    <rdf:Description rdf:about="http://erlangen-crm.org/efrbroo/F23_Expression_Fragment"/>
                </owl:intersectionOf>
            </owl:Class>
        </rdfs:subClassOf>
        <owl:disjointWith rdf:resource="http://purl.org/saws/ontology#Marginalia"/>
        <rdfs:comment xml:lang="en">Comment on a part of the material, usually from the modern editor. 

N.B. The Comment class is for comments on a material that do not physically exist on that material. If a comment has been physically written on a material (usually in the margin), then this should be represented as an instance of Marginalia. </rdfs:comment>
        <rdfs:label xml:lang="en">comment</rdfs:label>
    </owl:Class>
    


    <!-- http://purl.org/saws/ontology#ContentItem -->

    <owl:Class rdf:about="http://purl.org/saws/ontology#ContentItem">
        <rdfs:subClassOf>
            <owl:Class>
                <owl:intersectionOf rdf:parseType="Collection">
                    <rdf:Description rdf:about="http://erlangen-crm.org/current/E33_Linguistic_Object"/>
                    <rdf:Description rdf:about="http://erlangen-crm.org/efrbroo/F23_Expression_Fragment"/>
                </owl:intersectionOf>
            </owl:Class>
        </rdfs:subClassOf>
        <rdfs:comment xml:lang="en">A basic unit of interest within the Material: a division of a collection instance/section, for more exact reference than when using a section – this identifies basic units of interest in the material for SAWS (marked in TEI as &lt;seg&gt;)</rdfs:comment>
        <rdfs:label xml:lang="en">content item</rdfs:label>
    </owl:Class>
    


    <!-- http://purl.org/saws/ontology#DecorativeItem -->

    <owl:Class rdf:about="http://purl.org/saws/ontology#DecorativeItem">
        <rdfs:subClassOf rdf:resource="http://erlangen-crm.org/current/E36_Visual_Item"/>
        <rdfs:comment xml:lang="en">Decorative element (picture, ornamentation, etc) within the material, either meaning-bearing or non meaning-bearing</rdfs:comment>
        <rdfs:label xml:lang="en">decorative item</rdfs:label>
    </owl:Class>
    


    <!-- http://purl.org/saws/ontology#Definition -->

    <owl:Class rdf:about="http://purl.org/saws/ontology#Definition">
        <rdfs:subClassOf rdf:resource="http://purl.org/saws/ontology#ContentItem"/>
        <rdfs:comment xml:lang="en">A content item that is defining a concept or term used in the material</rdfs:comment>
        <rdfs:label xml:lang="en">definition</rdfs:label>
    </owl:Class>
    


    <!-- http://purl.org/saws/ontology#Edition -->

    <owl:Class rdf:about="http://purl.org/saws/ontology#Edition">
        <rdfs:subClassOf rdf:resource="http://purl.org/saws/ontology#Material"/>
        <owl:disjointWith rdf:resource="http://purl.org/saws/ontology#OriginalMaterial"/>
        <rdfs:comment xml:lang="en">Any edited material, known or unknown, including texts such as the Bible and Kekaumenos</rdfs:comment>
        <rdfs:label xml:lang="en">edition</rdfs:label>
    </owl:Class>
    


    <!-- http://purl.org/saws/ontology#Editor -->

    <owl:Class rdf:about="http://purl.org/saws/ontology#Editor">
        <rdfs:subClassOf rdf:resource="http://erlangen-crm.org/current/E21_Person"/>
        <owl:disjointWith rdf:resource="http://purl.org/saws/ontology#Scribe"/>
        <owl:disjointWith rdf:resource="http://purl.org/saws/ontology#Transmitter"/>
        <rdfs:comment xml:lang="en">A modern scholar editing material to produce an edition, in the age of printing and beyond</rdfs:comment>
        <rdfs:label xml:lang="en">editor</rdfs:label>
    </owl:Class>
    


    <!-- http://purl.org/saws/ontology#EditorSection -->

    <owl:Class rdf:about="http://purl.org/saws/ontology#EditorSection">
        <rdfs:subClassOf rdf:resource="http://purl.org/saws/ontology#Section"/>
        <owl:disjointWith rdf:resource="http://purl.org/saws/ontology#ScribeSection"/>
        <rdfs:comment xml:lang="en">Any division within a linguistic object created by an editor, e.g. to make the navigation of the text clearer or to mark a region of interest</rdfs:comment>
        <rdfs:label xml:lang="en">editor section</rdfs:label>
    </owl:Class>
    


    <!-- http://purl.org/saws/ontology#EditorTitle -->

    <owl:Class rdf:about="http://purl.org/saws/ontology#EditorTitle">
        <rdfs:subClassOf rdf:resource="http://erlangen-crm.org/current/E35_Title"/>
        <owl:disjointWith rdf:resource="http://purl.org/saws/ontology#ScribeTitle"/>
        <rdfs:comment xml:lang="en">Indicates a title that was assigned outside the manuscript by an editor</rdfs:comment>
        <rdfs:label xml:lang="en">editor title</rdfs:label>
    </owl:Class>
    


    <!-- http://purl.org/saws/ontology#Epilogue -->

    <owl:Class rdf:about="http://purl.org/saws/ontology#Epilogue">
        <rdfs:subClassOf rdf:resource="http://purl.org/saws/ontology#Section"/>
        <owl:disjointWith rdf:resource="http://purl.org/saws/ontology#Prologue"/>
        <rdfs:label xml:lang="en">epilogue</rdfs:label>
    </owl:Class>
    


    <!-- http://purl.org/saws/ontology#Family -->

    <owl:Class rdf:about="http://purl.org/saws/ontology#Family">
        <rdfs:subClassOf rdf:resource="http://erlangen-crm.org/efrbroo/F15_Complex_Work"/>
        <rdfs:comment xml:lang="en">A grouping of related Materials - this is a concept, an interpretation, rather than a physical thing</rdfs:comment>
        <rdfs:label xml:lang="en">family</rdfs:label>
    </owl:Class>
    


    <!-- http://purl.org/saws/ontology#HypothesisedInstance -->

    <owl:Class rdf:about="http://purl.org/saws/ontology#HypothesisedInstance">
        <rdfs:subClassOf rdf:resource="http://purl.org/saws/ontology#OriginalMaterial"/>
        <rdfs:subClassOf>
            <owl:Class>
                <owl:unionOf rdf:parseType="Collection">
                    <rdf:Description rdf:about="http://purl.org/saws/ontology#AbstractManuscriptText"/>
                    <rdf:Description rdf:about="http://purl.org/saws/ontology#CollectionInstance"/>
                </owl:unionOf>
            </owl:Class>
        </rdfs:subClassOf>
        <rdfs:comment xml:lang="en">The physical instance of an abstract manuscript text or collection instance which we hypothesise may have existed, but which we do not have - it is presumed lost or destroyed</rdfs:comment>
        <rdfs:label xml:lang="en">hypothesised instance</rdfs:label>
    </owl:Class>
    


    <!-- http://purl.org/saws/ontology#Institution -->

    <owl:Class rdf:about="http://purl.org/saws/ontology#Institution">
        <rdfs:subClassOf rdf:resource="http://erlangen-crm.org/current/E74_Group"/>
        <rdfs:comment xml:lang="en">An Institution can own materials, be located at places, and include persons as members</rdfs:comment>
        <rdfs:label xml:lang="en">institution</rdfs:label>
    </owl:Class>
    


    <!-- http://purl.org/saws/ontology#Lacuna -->

    <owl:Class rdf:about="http://purl.org/saws/ontology#Lacuna">
        <rdfs:subClassOf rdf:resource="http://erlangen-crm.org/current/E53_Place"/>
        <rdfs:comment xml:lang="en">A physical gap in the physical manuscript</rdfs:comment>
        <rdfs:label xml:lang="en">lacuna</rdfs:label>
    </owl:Class>
    


    <!-- http://purl.org/saws/ontology#Locus -->

    <owl:Class rdf:about="http://purl.org/saws/ontology#Locus">
        <rdfs:subClassOf rdf:resource="http://erlangen-crm.org/current/E53_Place"/>
        <rdfs:comment xml:lang="en">A physical location within a physical manuscript</rdfs:comment>
        <rdfs:label xml:lang="en">locus</rdfs:label>
    </owl:Class>
    


    <!-- http://purl.org/saws/ontology#ManuscriptPart -->

    <owl:Class rdf:about="http://purl.org/saws/ontology#ManuscriptPart">
        <rdfs:subClassOf rdf:resource="http://purl.org/saws/ontology#Locus"/>
        <rdfs:comment xml:lang="en">A physical section of a physical manuscript</rdfs:comment>
        <rdfs:label xml:lang="en">manuscript part</rdfs:label>
    </owl:Class>
    


    <!-- http://purl.org/saws/ontology#Marginalia -->

    <owl:Class rdf:about="http://purl.org/saws/ontology#Marginalia">
        <rdfs:subClassOf>
            <owl:Class>
                <owl:intersectionOf rdf:parseType="Collection">
                    <rdf:Description rdf:about="http://erlangen-crm.org/current/E33_Linguistic_Object"/>
                    <rdf:Description rdf:about="http://erlangen-crm.org/efrbroo/F23_Expression_Fragment"/>
                </owl:intersectionOf>
            </owl:Class>
        </rdfs:subClassOf>
        <rdfs:comment xml:lang="en">Remark(s) physically written in the margin of the material by a scribe, not necessarily the original scribe. 

N.B. If a comment has been physically written on a material (usually in the margin), then this should be represented as an instance of Marginalia. The Comment class is for comments on a material that don’t physically exist on that material</rdfs:comment>
        <rdfs:label xml:lang="en">marginalia</rdfs:label>
    </owl:Class>
    


    <!-- http://purl.org/saws/ontology#Material -->

    <owl:Class rdf:about="http://purl.org/saws/ontology#Material">
        <rdfs:subClassOf>
            <owl:Class>
                <owl:intersectionOf rdf:parseType="Collection">
                    <rdf:Description rdf:about="http://erlangen-crm.org/current/E33_Linguistic_Object"/>
                    <rdf:Description rdf:about="http://erlangen-crm.org/efrbroo/F22_Self-Contained_Expression"/>
                </owl:intersectionOf>
            </owl:Class>
        </rdfs:subClassOf>
        <rdfs:comment xml:lang="en">Any of the texts we are working on in SAWS or that we are referring to</rdfs:comment>
        <rdfs:label xml:lang="en">material</rdfs:label>
    </owl:Class>
    


    <!-- http://purl.org/saws/ontology#Narrative -->

    <owl:Class rdf:about="http://purl.org/saws/ontology#Narrative">
        <rdfs:subClassOf rdf:resource="http://purl.org/saws/ontology#ContentItem"/>
        <rdfs:comment xml:lang="en">Narrative text that is not a saying itself, that either stands alone or is the text surrounding or immediately preceding or following the Statement (saying), e.g. &apos;Aristotle says...&apos;, &apos;The frogs asked for a king.’, ‘Aristotle is a lover of knowledge’</rdfs:comment>
        <rdfs:label xml:lang="en">narrative</rdfs:label>
    </owl:Class>
    


    <!-- http://purl.org/saws/ontology#OriginalMaterial -->

    <owl:Class rdf:about="http://purl.org/saws/ontology#OriginalMaterial">
        <rdfs:subClassOf rdf:resource="http://purl.org/saws/ontology#Material"/>
        <rdfs:comment xml:lang="en">A material produced by scribe transcription rather than being edited in modern times</rdfs:comment>
        <rdfs:label xml:lang="en">original material</rdfs:label>
    </owl:Class>
    


    <!-- http://purl.org/saws/ontology#OtherContentItem -->

    <owl:Class rdf:about="http://purl.org/saws/ontology#OtherContentItem">
        <rdfs:subClassOf rdf:resource="http://purl.org/saws/ontology#ContentItem"/>
        <rdfs:comment xml:lang="en">A unit of the material within a content item, as identified by the modern editor, which isn’t a narrative, statement, or definition</rdfs:comment>
        <rdfs:label xml:lang="en">other content item</rdfs:label>
    </owl:Class>
    


    <!-- http://purl.org/saws/ontology#PhysicalManuscript -->

    <owl:Class rdf:about="http://purl.org/saws/ontology#PhysicalManuscript">
        <rdfs:subClassOf rdf:resource="http://erlangen-crm.org/efrbroo/F4_Manifestation_Singleton"/>
        <owl:disjointWith rdf:resource="http://purl.org/saws/ontology#ReconstructedManuscript"/>
        <rdfs:comment xml:lang="en">The physical object on which the material we are working on exists</rdfs:comment>
        <rdfs:label xml:lang="en">physical manuscript</rdfs:label>
    </owl:Class>
    


    <!-- http://purl.org/saws/ontology#Prologue -->

    <owl:Class rdf:about="http://purl.org/saws/ontology#Prologue">
        <rdfs:subClassOf rdf:resource="http://purl.org/saws/ontology#Section"/>
        <rdfs:label xml:lang="en">prologue</rdfs:label>
    </owl:Class>
    


    <!-- http://purl.org/saws/ontology#ReconstructedManuscript -->

    <owl:Class rdf:about="http://purl.org/saws/ontology#ReconstructedManuscript">
        <rdfs:subClassOf rdf:resource="http://erlangen-crm.org/efrbroo/F4_Manifestation_Singleton"/>
        <rdfs:comment xml:lang="en">Manuscript whose parts are now distributed as separate manuscript parts, so no longer exists as a whole, but can still be identified</rdfs:comment>
        <rdfs:label xml:lang="en">reconstructed manuscript</rdfs:label>
    </owl:Class>
    


    <!-- http://purl.org/saws/ontology#Scribe -->

    <owl:Class rdf:about="http://purl.org/saws/ontology#Scribe">
        <rdfs:subClassOf rdf:resource="http://erlangen-crm.org/current/E21_Person"/>
        <rdfs:comment xml:lang="en">The producer / author / copier of a linguistic object (excluding editions), in the medieval age. The scribe can be named or unnamed</rdfs:comment>
        <rdfs:label xml:lang="en">scribe</rdfs:label>
    </owl:Class>
    


    <!-- http://purl.org/saws/ontology#ScribeSection -->

    <owl:Class rdf:about="http://purl.org/saws/ontology#ScribeSection">
        <rdfs:subClassOf rdf:resource="http://purl.org/saws/ontology#Section"/>
        <rdfs:comment xml:lang="en">Any division within a linguistic object indicated by a scribe</rdfs:comment>
        <rdfs:label xml:lang="en">scribe section</rdfs:label>
    </owl:Class>
    


    <!-- http://purl.org/saws/ontology#ScribeTitle -->

    <owl:Class rdf:about="http://purl.org/saws/ontology#ScribeTitle">
        <rdfs:subClassOf rdf:resource="http://erlangen-crm.org/current/E35_Title"/>
        <rdfs:comment xml:lang="en">Indicates a title that was assigned within the manuscript by a scribe</rdfs:comment>
        <rdfs:label xml:lang="en">scribe title</rdfs:label>
    </owl:Class>
    


    <!-- http://purl.org/saws/ontology#Section -->

    <owl:Class rdf:about="http://purl.org/saws/ontology#Section">
        <rdfs:subClassOf>
            <owl:Class>
                <owl:intersectionOf rdf:parseType="Collection">
                    <rdf:Description rdf:about="http://erlangen-crm.org/current/E33_Linguistic_Object"/>
                    <rdf:Description rdf:about="http://erlangen-crm.org/efrbroo/F22_Self-Contained_Expression"/>
                </owl:intersectionOf>
            </owl:Class>
        </rdfs:subClassOf>
        <rdfs:comment xml:lang="en">A division of a linguistic object e.g. chapter, verse, for larger-scale reference than when using a content item. These can be nested/numbered</rdfs:comment>
        <rdfs:label xml:lang="en">section</rdfs:label>
    </owl:Class>
    


    <!-- http://purl.org/saws/ontology#Statement -->

    <owl:Class rdf:about="http://purl.org/saws/ontology#Statement">
        <rdfs:subClassOf rdf:resource="http://purl.org/saws/ontology#ContentItem"/>
        <rdfs:comment xml:lang="en">The actual saying, e.g. &apos;All men are mortal&apos;</rdfs:comment>
        <rdfs:label xml:lang="en">statement</rdfs:label>
    </owl:Class>
    


    <!-- http://purl.org/saws/ontology#Transmitter -->

    <owl:Class rdf:about="http://purl.org/saws/ontology#Transmitter">
        <rdfs:subClassOf rdf:resource="http://erlangen-crm.org/current/E21_Person"/>
        <rdfs:comment xml:lang="en">Person who is described in the text content as having transmitted a content item or other linguistic objects, for example ‘[Transmitter] said that [AttributedAuthor] said … (ContentItem)</rdfs:comment>
        <rdfs:label xml:lang="en">transmitter</rdfs:label>
    </owl:Class>
    


    <!-- 
    ///////////////////////////////////////////////////////////////////////////////////////
    //
    // Annotations
    //
    ///////////////////////////////////////////////////////////////////////////////////////
     -->

    <rdf:Description rdf:about="http://erlangen-crm.org/current/E39_Actor">
        <rdfs:comment xml:lang="en">Note for SAWS: we can use Actor to refer to any living being (not necessarily a person, not necessarily still alive) who is identified/named/referred to within a linguistic object, though we may wish to use a more specific class such as Person, AttributedAuthor, Scribe etc.</rdfs:comment>
        <rdfs:label xml:lang="en">actor</rdfs:label>
    </rdf:Description>
    <rdf:Description rdf:about="http://erlangen-crm.org/current/E41_Appellation">
        <rdfs:label xml:lang="en">appellation</rdfs:label>
        <rdfs:comment xml:lang="en">Note for SAWS: we can use Appellation to state a person’s name or other name of interest e.g. of a church</rdfs:comment>
    </rdf:Description>
    <rdf:Description rdf:about="http://erlangen-crm.org/current/E51_Contact_Point">
        <rdfs:label xml:lang="en">contact point</rdfs:label>
    </rdf:Description>
    


    <!-- 
    ///////////////////////////////////////////////////////////////////////////////////////
    //
    // General axioms
    //
    ///////////////////////////////////////////////////////////////////////////////////////
     -->

    <rdf:Description>
        <rdf:type rdf:resource="http://www.w3.org/2002/07/owl#AllDisjointClasses"/>
        <owl:members rdf:parseType="Collection">
            <rdf:Description rdf:about="http://purl.org/saws/ontology#Definition"/>
            <rdf:Description rdf:about="http://purl.org/saws/ontology#Narrative"/>
            <rdf:Description rdf:about="http://purl.org/saws/ontology#OtherContentItem"/>
            <rdf:Description rdf:about="http://purl.org/saws/ontology#Statement"/>
        </owl:members>
    </rdf:Description>
</rdf:RDF>



<!-- Generated by the OWL API (version 4.5.9.2019-02-01T07:24:44Z) https://github.com/owlcs/owlapi -->

